cleanup 1

thorin/semantics/lang.v
@@ -1,94 +1,14 @@
 From stdpp Require Export binders strings.
 From iris.prelude Require Import options.
 From thorin.lib Require Export maps.
+Require Import Coq.Program.Equality.
 
 Declare Scope expr_scope.
 Declare Scope val_scope.
 Delimit Scope expr_scope with E.
 Delimit Scope val_scope with V.
 
-(*
-
-open conceptual TODO:
-- some missing assumptions/mistakes in the pdf
-- is a lam with normalized type also a value or only if the type is evaluated (a value)
-- recheck: normalization is no subset of evaluation (normalization goes under binders)
-  - does normalization go under binder?
-- TODO: how to formalize normalization
-- does order (left-to-right, bottom-up) matter for normalization
-- ----
-- the proof are technically hard:
-  - mutual induction with assignability
-  - nested induction with the lists
-  - normalization in between on type level
-- name clashes for substitutivity
-- is a variable a value? if not, it is not progressing
-- typing does normalization => base step preservation needs to argue that type already normalized or we need to normalize again
-- preservation of the form "if typed, then normalized is value or steps"?
-
-
-
-Normalization:
-- pre-requirement for reduction
-- not performed in reduction currently (we always argue about one reduction step)
-  - we can assert normalize before and conceptually normalize afterward
-- currently, 
-
-
-λ (x:T) : U @ef, eb
-we do not reduce under binders => only redex is T
-we use λ in app if T is normalized
-=> TODO: is_val should be true if T is normalized
-hence, we conceptually (and practically) only reduce until T is normalized
-but by construction, T is normalized
-=> TODO: a few consequences
-- on type level, normalization is our value relation
-- is_val should rely on normalized
-- relation to beta
-  - (without norm as pre-op, norm should not go under binders)
-  - 'beta reduce until norm' does not really hold (and if so only if not under binder)
-- TODO: there should not be any type reduxes (except maybe toplevel?)
-  - no redex in the type of a lambda
-  - same with sigma
-  - can Pi have a redex => should have, right?
-
-
-
-
-
-A short outline of the document.
-Each part has its own comments with relevant explanations.
-
-Outline lang.v:
-- expr -- Expression type of thorin
-- is_val
-- subst
-- normalize_step -- a single toplevel normalization step according to ▹
-- full_ectx -- Full contexts going through binders
-- full_contextual_step -- doing a step under a context
-- normal_eval -- predicate to relate an expression to its normal(ized) form
-- base_step -- a single toplevel reduction step
-- ectx -- evaluation contexts for reductino
-- contextual_step -- step under a context
-- contextual_step lemmas -- if subexpression steps, whole expression steps
-
-Outline types_sol.v:
-- syn_typed -- typing derivation, assignability relation
-- typed_weakening -- we can extend the context
-- typed_substitutivity -- subst in context, expression, type
-- canonical value lemma -- if value has some type, it has some shape
-- typed_progress -- typed expressions can reduce or are a value (TODO: needs normalization)
-- typed_preservation_base_step -- a toplevel reduction preserves types
-- typed_preservation -- preservation over multiple steps
-
-*)
-
-
-
-
 Inductive expr :=
-  (* | Star
-  | Box *)
   | Sort (n:nat)
   | Bot
   | Nat
@@ -99,41 +19,12 @@ Inductive expr :=
   (* let is already normalized *)
   (* axiom is already handled *)
   | Pi (x : binder) (T U : expr)
-  (* lam has a filter expression *)
   | Lam (x : binder) (T : expr) (f : expr) (U: expr) (e: expr)
   | App (e1 e2 : expr)
-  (* | Sigma (args: list (binder * expr))
-  | Tuple (es : list expr)
-  | Array (x: binder) (en: expr) (T: expr)
-  | Pack (x: binder) (en: expr) (e: expr)
-  | Extract (e: expr) (ei: expr) *)
 .
 
 Bind Scope expr_scope with expr.
 
-(*
-  We argue at some points over lists.
-  We could use ∀x∈xs. P x
-  However, we want a stronger statement:
-  - Computational (not Prop)
-  - List structure linked to xs
-  - Able to use induction/destructuring on the strucutre
-
-  https://ps.uni-saarland.de/~ullrich/bachelor.php
-  https://github.com/NeuralCoder3/parametricity-note
-
-  We use the unary ∀ parametricity relation
-  For lists, this is Forall.
-*)
-
-
-(* 
-  Semantics uses an additional val type with of_val, to_val and conversions between them.
-  They need it to simplify the definition of computational steps (e.g. un_op_eval/bin_op_eval). (but not significantly)
-
-  To me, a inductive predicate is_val seems to be shorter and simpler.
-  All our proofs only argue about is_val.
-*)
 
 Fixpoint subst (x : string) (es : expr) (e : expr)  : expr :=
   let recurse_under y expr := if decide (y = BNamed x) then expr else subst x es expr in
@@ -150,37 +41,11 @@ Fixpoint subst (x : string) (es : expr) (e : expr)  : expr :=
       (recurse_under y U)
       (recurse_under y e)
   | App e1 e2 => App (subst x es e1) (subst x es e2)
-  (* map over nested induction 
-  => use inner fixpoint 
-  mutual recursion is not recognized (https://coq.discourse.group/t/mutual-recursion-for-nested-inductive-types/729/3)
-  Equations would be possible but not necessarily easier
-   *)
-  (* | Tuple expression =>
-    Tuple (map (subst x es) expression)
-  (* for Sigma, we only continue subst in args if not already encountered var *)
-  | Sigma xs =>
-    Sigma ((fix fold_subst (xs : list (binder * expr)) : list (binder * expr) :=
-      match xs with
-      | [] => []
-      | (y, T) :: xs => 
-        (* stop at [x:..., ...] => later x are regarding the parameter*)
-        (y, subst x es T) :: (if decide (y = BNamed x) then xs else fold_subst xs)
-      end) xs)
-  | Array y en T => Array y (subst x es en) (recurse_under y T)
-  | Pack y en e => Pack y (subst x es en) (recurse_under y e)
-  | Extract e ei => Extract (subst x es e) (subst x es ei) *)
   end.
 
 Definition subst' (mx : binder) (es : expr) : expr → expr :=
   match mx with BNamed x => subst x es | BAnon => id end.
 
-(* Notation "e . [ x / e2 ]" := (subst x e2 e) (at level 20). *)
-(* Notation "e '.' '[' e2 '/' x ']'" := (subst' x e2 e) (at level 20).
-Check (Lam (BNamed "x") Nat (Var "x") Nat (Var "x")).[LitNat 3 / "x"]. *)
-
-
-
-Require Import Coq.Program.Equality.
 
 Lemma fin_inc n (i:Fin.t n): (` (Fin.to_nat (Fin.FS i))) = S (` (Fin.to_nat i)).
 Proof.
@@ -249,8 +114,6 @@ Inductive normalized : expr -> Prop :=
   (* atomic values *)
   (* conceptually, every value is normalized (not quite -- normalization goes under binders) *)
   (* but for distinction, differences and adaptation, we should keep normalization without is_val *)
-  (* | norm_Star: normalized Star
-  | norm_Box: normalized Box *)
   | norm_Sort n: normalized (Sort n)
   | norm_Bot: normalized Bot
   | norm_Nat: normalized Nat
@@ -269,107 +132,13 @@ Inductive normalized : expr -> Prop :=
   *)
   | norm_App e1 e2:
     normalized e1 -> normalized e2 -> 
-    (* TODO: not = ETrue but beta equiv to True *)
     ~(exists x T f U e, e1 = Lam x T f U e /\ f = ETrue) ->
     normalized (App e1 e2)
-
-  (*
-    Sigma
-    - subexpressions normalized
-    - not unary
-    - no unnamed array sigma [T, ..., T]
-  *)
-  (* | norm_Sigma xs:
-    (* without map separately, it would be a not strictly positive occurence of normalized *)
-    Forall normalized (map (fun '(x,T) => T) xs) ->
-    xs = [] \/ length xs > 1 ->
-    ~ (length xs > 1 /\ exists T, Forall (fun b => b = (BAnon, T)) xs) ->
-    normalized (Sigma xs)
-
-  (* Tuple
-    - subexpressions normalized 
-    - not unary 
-    - not eta tuple (e#i, i in 0..n-1) 
-    - not pack tuple (e, ..., e) 
-  *)
-  | norm_Tuple es:
-    Forall normalized es ->
-    es = [] \/ length es > 1 ->
-    ~ (length es > 1 /\ 
-      exists e, 
-        Forall2 (fun ei idx => ei = Extract e (LitIdx (length es) idx))
-          es (let (xs,_) := fin_list (length es) in xs)
-    ) ->
-    ~ (length es > 1 /\ exists e, es = replicate (length es) e) ->
-    normalized (Tuple es)
-
-  (*
-    Array
-    - subexpressions normalized
-    - no named & nat size
-  *)
-  | norm_Array x en T:
-    normalized en -> normalized T -> 
-    ~ (exists s n, x = BNamed s /\ en = LitNat n) ->
-    normalized (Array x en T)
-
-  (*
-    Pack
-    - subexpressions normalized
-    - no named & nat size
-  *)
-  | norm_Pack x en e:
-    normalized en -> normalized e -> 
-    ~ (exists s n, x = BNamed s /\ en = LitNat n) ->
-    normalized (Pack x en e)
-
-  (*
-    Extract
-    - subexpressions normalized
-    - no extract 0_1
-    - no extract of tuple with idx
-    - no extract of unnamed pack
-  *)
-  | norm_Extract e ei:
-    normalized e -> normalized ei -> 
-    ~ (ei = LitIdx 1 Fin.F1) ->
-    ~ (exists es idx, e = Tuple es /\ ei = LitIdx (length es) idx) ->
-    ~ (exists en eb, e = Pack BAnon en eb) ->
-    normalized (Extract e ei) *)
   .
 
 
-(* TODO: require normalized subexpressions? (would be needed for in-to-out-order) *)
 Inductive normalize_step : expr -> expr -> Prop :=
-  (* no let *)
-  (* | normalize_extract_one e:
-    (* TODO: need normalized of e? *)
-    normalize_step (Extract e (LitIdx 1 Fin.F1)) e
-  | normalize_tuple_one e:
-    normalize_step (Tuple [e]) e
-  | normalize_sigma_one x T:
-    normalize_step (Sigma [(x,T)]) T
-    (* normalize_step (Sigma [xT]) (Sigma [xT]) *)
-  | normalize_tuple_beta xs n i e:
-    length xs = n ->
-    nth_error xs (` (Fin.to_nat i)) = Some e ->
-    (* TODO: maybe we could model this using vectors *)
-    normalize_step (Extract (Tuple xs) (LitIdx n i)) e
-  | normalize_pack_beta en e ei:
-    normalize_step (Extract (Pack BAnon en e) ei) e
-  | normalize_tuple_eta e n:
-    (* TODO: n>1 missing from paper *)
-    n > 1 ->
-    normalize_step (Tuple (map (fun i => Extract e (LitIdx n i)) (ltac: (destruct (fin_list n) as [xs _];exact xs)))) e
-  | normalize_pack_tuple n e:
-    (* replicate is the same as repeat *)
-    n > 1 ->
-    normalize_step (Tuple (replicate n e)) (Pack (BAnon) (LitNat n) e)
-  | normalize_array_sigma n T:
-    n > 1 ->
-    normalize_step (Sigma (replicate n (BAnon, T))) (Array (BAnon) (LitNat n) T) *)
   | normalize_beta x T ef U eb ea:
-    (* TODO: ef[ea/x] beta equiv true *)
     ef = ETrue ->
     normalized T ->
     normalized U ->
@@ -377,19 +146,8 @@ Inductive normalize_step : expr -> expr -> Prop :=
     normalized eb ->
     normalized ea ->
     normalize_step (App (Lam x T ef U eb) ea) (subst' x ea eb)
-  (* | normalize_tuple_pack x n e:
-    normalize_step (Pack (BNamed x) (LitNat n) e) (Tuple (instantiate x n e))
-  | normalize_sigma_array x n T:
-    normalize_step (Array (BNamed x) (LitNat n) T) (Sigma (map (fun x => (BAnon, x)) (instantiate x n T)))
-
-  (* TODO: not in paper *)
-  | normalize_pack_one e:
-    normalize_step (Pack BAnon (LitNat 1) e) e
-  | normalize_array_one T:
-    normalize_step (Array BAnon (LitNat 1) T) T *)
 .
 
-(* TODO: do we need to require left-to-right or in-to-out order? *)
 Inductive full_ectx :=
   | FHoleCtx
   | FPi1 (x:binder) (K: full_ectx) (U:expr)
@@ -400,14 +158,6 @@ Inductive full_ectx :=
   | FLam4 (x:binder) (T: expr) (f:expr) (U:expr) (e:full_ectx)
   | FApp1 (K: full_ectx) (e2 : expr)
   | FApp2 (e1 : expr) (K: full_ectx)
-  (* | FSigma (xs1: list (binder * expr)) (x:binder) (K: full_ectx) (xs2: list (binder * expr))
-  | FTuple (es1:list expr) (K: full_ectx) (es2: list expr)
-  | FArray1 (x:binder) (en: full_ectx) (T:expr)
-  | FArray2 (x:binder) (en: expr) (T: full_ectx)
-  | FPack1 (x:binder) (en: full_ectx) (e:expr)
-  | FPack2 (x:binder) (en: expr) (e: full_ectx)
-  | FExtract1 (K: full_ectx) (ei:expr)
-  | FExtract2 (e:expr) (K: full_ectx) *)
   .
 
 Fixpoint full_fill (K:full_ectx) (e:expr) : expr :=
@@ -421,14 +171,6 @@ Fixpoint full_fill (K:full_ectx) (e:expr) : expr :=
   | FLam4 x T f U K  => Lam x T f U (full_fill K e)
   | FApp1 K e2 => App (full_fill K e) e2
   | FApp2 e1 K => App e1 (full_fill K e)
-  (* | FSigma xs1 x K xs2 => Sigma (xs1 ++ (x,full_fill K e) :: xs2)
-  | FTuple es1 K es2 => Tuple (es1 ++ full_fill K e :: es2)
-  | FArray1 x K T => Array x (full_fill K e) T
-  | FArray2 x en K => Array x en (full_fill K e)
-  | FPack1 x K eb => Pack x (full_fill K e) eb
-  | FPack2 x en K => Pack x en (full_fill K e)
-  | FExtract1 K ei => Extract (full_fill K e) ei
-  | FExtract2 eb K => Extract eb (full_fill K e) *)
   end.
 
 Fixpoint comp_full_ectx (K1 K2: full_ectx) :=
@@ -448,71 +190,30 @@ Lemma full_fill_comp K1 K2 e:
   full_fill (comp_full_ectx K1 K2) e = full_fill K1 (full_fill K2 e).
 Proof. induction K1; simpl; congruence. Qed.
 
-(* Definition normalizable (e : expr) :=
-  ∃ e', full_contextual_step e e'. *)
-
-(* Inductive full_contextual_step (e1 : expr) (e2 : expr) : Prop :=
-  Fectx_step K (e1_lam' e1_arg':expr) e2' :
-  (* maybe normalized e1' and e2' already *)
-    e1 = full_fill K (App e1_lam' e1_arg') → 
-    e2 = full_fill K e2' →
-    normalize_step (App e1_lam' e1_arg') e2' → 
-    full_contextual_step e1 e2
-with normalized_pred (e : expr) :=
-  | norm_pred : ~ (∃ e', full_contextual_step e e') -> normalized_pred e. *)
-
-
-(* Fixpoint full_contextual_step (e1 : expr) (e2 : expr) : Prop :=
-  exists K e1' e2',
-    normalized e1' ∧
-    e1 = full_fill K e1' ∧ e2 = full_fill K e2' ∧ normalize_step e1' e2'
-with normalized_pred (e:expr) := ~ exists e', full_contextual_step e e'. *)
-
-
 Inductive full_contextual_step (e1 : expr) (e2 : expr) : Prop :=
+  (* by the definition of normalize_step, the subexpressions are already normalized
+    enforcing full normalization from bottom up
+  *)
   Fectx_step K e1' e2' :
-  (* maybe normalized e1' and e2' already *)
-    e1 = full_fill K e1' → e2 = full_fill K e2' →
-    (* normalized_pred (full_contextual_step) e1' →  *)
-    normalize_step e1' e2' → full_contextual_step e1 e2.
-
-(* Definition normalized_pred (step:expr -> expr -> Prop) (e : expr) :=
-  ~ ∃ e', step e e'. *)
-
-
-(* Inductive full_contextual_step (e1 : expr) (e2 : expr) : Prop :=
-  Fectx_step K e1' e2' :
-  (* maybe normalized e1' and e2' already *)
     e1 = full_fill K e1' → e2 = full_fill K e2' →
     normalize_step e1' e2' → full_contextual_step e1 e2.
 
-Definition normalized_pred (e : expr) :=
-  ~ ∃ e', full_contextual_step e e'. *)
+(*
+Due to indirection, a inductive definition is not possible
+This version (using ~∃) is a pain to work with.
+We will usually use the constructive inductive predicate
+but this formulation is more direct / related to the code
+*)
 Definition normalized_pred (e : expr) :=
   ~ ∃ e', full_contextual_step e e'.
 
-  (* maybe as inductive? *)
-  (* perform all possible normalization redexes *)
+(* perform all possible normalization redexes *)
 Definition normal_eval e e' :=
   rtc full_contextual_step e e' ∧ normalized_pred e'.
 
-(*
-  a bit more constructive version
-  => subexpressions and contradict normalization step in negative assumptions
-
-
-  TODO: change
-*)
-(* TODO:
-  enumerate full constructive (as far as possible) normalized predicate
-  TODO: not up to date
-
-
+(* 
   we define is_val for normalized expressions => does not contain a beta redex
-  we do not go into types of dependencies (only decent along evaluation contexts)
-  but we descend under binders
-
-  applications and extracts are not values
+  applications are not values
 *)
 Definition is_lam (e:expr) :=
   match e with
@@ -520,22 +221,16 @@ Definition is_lam (e:expr) :=
   | _ => False
   end.
 Inductive is_val : expr → Prop :=
-(* with is_val : expr → Prop := *)
-  (* atomic values *)
-  (* | StarV : is_val Star
-  | BoxV : is_val Box *)
-  (* or talk about closed for preservation *)
-  (* Var should not be value otherwise, we destroy canonical value lemmas *)
+  (* progress in CC needs to talk about vars *)
+  (* we do not have canonical values directly as we need vars as values *)
   | VarV x : is_val (Var x) 
   | AppV v1 v2: 
-    (* not lambda *)
     ~is_lam v1 →
     is_val v1 → is_val v2 → is_val (App v1 v2)
   | SortV n : is_val (Sort n)
   | BotV : is_val Bot
   | NatV : is_val Nat
   | IdxV : is_val Idx
-  (* TODO: is (Idx n) a value? if not what does it reduce to *)
   | IdxAppV n : is_val (App Idx (LitNat n))
   | LitNatV n : is_val (LitNat n)
   | LitIdxV n i : is_val (LitIdx n i)
@@ -544,38 +239,11 @@ Inductive is_val : expr → Prop :=
     is_val U →
     is_val (Pi x T U)
   | LamV x T f U e : 
-    (* TODO: should this be value or normalized?
-    => we step not in the type
-    => normalization already sufficient for value
-     *)
     is_val T →
     is_val U →
-    (* normalized T → *)
     (* U might depend on x:T *)
     is_val e ->
     is_val (Lam x T f U e)
-  (* compound values *)
-  (* 
-    sigma is like lambda (functions depending on previous values)
-    => only the first one should be a val
-  *)
-  (* | SigmaV xs: is_val (Sigma xs)
-  (* | SigmaEmptyV: is_val (Sigma [])
-  (* we do not need to test the rest => (implicitely) depends on first one *)
-  | SigmaConsV x T args : 
-    (* same as lambda *)
-    (* is_val T →  *)
-    (* normalized T → *)
-    is_val (Sigma ((x, T) :: args)) *)
-  | TupleV es : Forall is_val es → is_val (Tuple es)
-  | ArrayV x en T : 
-    (* is_val en →
-    is_val T → *)
-    is_val (Array x en T)
-  | PackV x en e :
-    is_val en →
-    is_val e →
-    is_val (Pack x en e) *)
   .
 
 
@@ -584,9 +252,7 @@ Lemma norm_sound e:
 Proof.
   induction 1.
   all:unfold normalized_pred;intros [e' Hstep].
-  (* all: revert Hstep. *)
   all:inversion Hstep;subst.
-  (* all: revert H. *)
   1-7: destruct K;simpl in *;inversion H;subst.
   1-7: now inversion H1.
   1: {
@@ -636,11 +302,6 @@ Proof.
       econstructor;eauto.
   }
 Qed.
-
-
-
-(* Lemma norm_total e:
-  exists e', e →ₙ e'. *)
 
 
 Lemma norm_sound2 e: 
@@ -695,204 +356,23 @@ Proof.
 Qed.
 
 
-(* Lemma normalized_sound e:
-  (* normalized_pred := ~ normalizable *)
-  normalized e -> ~ normalizable e.
-Proof.
-  induction 1;intros [e' Hnorm].
-  1-8: (
-    destruct Hnorm;subst;
-    destruct K;simpl in *;inversion H;subst;
-    inversion H1
-  ).
-  (* 
-  - (* Star *)
-    destruct Hnorm;subst.
-    destruct K;simpl in *;inversion H;subst.
-    inversion H1.
-  *)
-  (* - admit.
-  - admit.
-  - admit.
-  - admit.
-  - admit.
-  - admit.
-  - admit. *)
-  (*
-    we look at the normalization step and context
-    => is the context toplevel or a subexpression
-    for toplevel: which normalization step
-      each normalization step contradicted by assumption
-    each subexpression contradiction
-  *)
-  - (* Pi *)
-    destruct Hnorm;subst.
-    destruct K;simpl in *;inversion H1;subst.
-    + inversion H3. (* Pi does not make a norm step *)
-    + contradict IHnormalized1.
-      eexists.
-      econstructor;eauto.
-    + contradict IHnormalized2.
-      eexists.
-      econstructor;eauto.
-  - (* Lam -- similar to Pi *)
-    destruct Hnorm;subst.
-    destruct K;simpl in *;inversion H3;subst.
-    + inversion H5.
-    + contradict IHnormalized1;eexists;econstructor;eauto.
-    + contradict IHnormalized2;eexists;econstructor;eauto.
-    + contradict IHnormalized3;eexists;econstructor;eauto.
-    + contradict IHnormalized4;eexists;econstructor;eauto.
-  - (* App *)
-    destruct Hnorm;subst.
-    destruct K;simpl in *;inversion H2;subst.
-    + inversion H4;subst.
-      contradict H1.
-      do 5 eexists;eauto.
-    + contradict IHnormalized1.
-      eexists.
-      econstructor;eauto.
-    + contradict IHnormalized2.
-      eexists.
-      econstructor;eauto.
-  - (* Sigma *)
-    destruct Hnorm;subst.
-    destruct K;simpl in *;inversion H2;subst.
-    + inversion H4;subst.
-      * (* unary Sigma *)
-        simpl in H0.
-        destruct H0;try congruence.
-        lia.
-      * (* replicate *)
-        contradict H1.
-        split.
-        -- now rewrite replicate_length.
-        -- exists T. admit. (* easy *)
-    + admit. (* needs nested induction *)
-  - (* Tuple *)
-    destruct Hnorm;subst.
-    destruct K;simpl in *;inversion H3;subst.
-    + inversion H5;subst.
-      * destruct H0;eauto. inversion H0.
-      * contradict H1.
-        admit.
-      * contradict H2. split.
-        -- rewrite replicate_length. easy.
-        -- rewrite replicate_length. eauto.
-    + admit. (* needs nested induction *)
-  - (* Array *)
-    destruct Hnorm;subst.
-    destruct K;simpl in *;inversion H2;subst.
-    + inversion H4;subst.
-      contradict H1.
-      eauto.
-    + contradict IHnormalized1;eexists;econstructor;eauto.
-    + contradict IHnormalized2;eexists;econstructor;eauto.
-  - (* Pack *)
-    destruct Hnorm;subst.
-    destruct K;simpl in *;inversion H2;subst.
-    + inversion H4;subst.
-      contradict H1. eauto.
-    + contradict IHnormalized1;eexists;econstructor;eauto.
-    + contradict IHnormalized2;eexists;econstructor;eauto.
-  - (* Extract *) 
-    destruct Hnorm;subst.
-    destruct K;simpl in *;inversion H4;subst.
-    + inversion H6;subst.
-      * now contradict H1.
-      * contradict H2. eauto.
-      * contradict H3. eauto.
-    + contradict IHnormalized1;eexists;econstructor;eauto.
-    + contradict IHnormalized2;eexists;econstructor;eauto.
-Admitted. *)
-
-
-
-
-
-
-
-
-
-
-
-
 (*
-Importantly, we do not evaluate on type level, we just normalize
-normalization is a subset/prestep of full evaluation
-
-on expression level, we want full eager (cbv) eval => values
-
-TODO: where to apply normalization?
-As extra reduction step (+normalized requirement?)? As separate step in between?
+our beta does not require normalization/evaluation per se (although every applicable expression will be normalized)
 *)
-
-
-(* https://coq.inria.fr/doc/v8.18/refman/language/core/conversion.html *)
+(* also see https://coq.inria.fr/doc/v8.18/refman/language/core/conversion.html *)
 Inductive base_step : expr -> expr -> Prop :=
-(* 'real' steps (congruence steps later) *)
+(* 'real' steps (congruence steps later via contexts) *)
   | BetaS x T f U elam earg e' :
-    (* not necessary if we only define beta on normalized terms *)
-    (* normalized T ->  *)
-    (* is_val earg -> *)
     e' = subst' x earg elam ->
     base_step (App (Lam x T f U elam) earg) e'
-  (* | IotaTupleS es n (i:Fin.t n) e:
-    (* extract from a tuple if all value *)
-    (* needs canonical form lemma for Idx n *)
-    (*
-    for nth, we need a proof about the size
-    alternatively, a vector would work but we would have the size everywhere
-    *)
-    (*
-    TODO: need normalization here?
-    *)
-    Forall is_val es ->
-    length es = n ->
-    nth_error es (` (Fin.to_nat i)) = Some e ->
-    base_step (Extract (Tuple es) (LitIdx n i)) e
-  (* extract of pack *)
-  | IotaPackS x e en ei e':
-    is_val ei -> (* implies ei = LitIdx n i (via canonical values?) *)
-    e' = subst' x ei e ->
-    (* TODO: do we need LitNat here or any arbitrary en? *)
-    (* base_step (Extract (Pack x (LitNat n) e) ei) e' *)
-    base_step (Extract (Pack x en e) ei) e' *)
   .
 
+
 (*
-  Extracts covered by normalization
-  for <x:en, e> # ei => e[ei/x]
-  we have a rule if en = n or x=_
-  we reach either case eventually
-
-  beta goes under binder
-*)
-
-
-(* evaluation contexts for congruence reduction *)
-(* a hole/context is an evaluation point *)
-(*
-  one difference is that semantics uses val to restrict the contexts
-  to an evaluation from right to left
-  We use additional is_val to restrict the contexts (should be correct here)
-
-  only relevant for two sided reductions in app, extract, and tuple
-
-  Note: we are a bit lazier => do not evaluate under binders
-
-
-  Change: we go under binders but not in types of dependencies => might lead to untyped code (no step in context necessary)
-  for dependent code, normalization is sufficient for our usage
+We go in every subexpression and under binder
 *)
 Inductive ectx :=
   | HoleCtx
-  (* only context in T as U might depend on x:T *)
-  (* | PiCtx (x:binder) (K: ectx) (U:expr)  *)
-  (* no, instead don't go under types *)
-  (* the filter depends on the argument *)
-  (* | LamCtx (x:binder) (K: ectx) (f:expr) (U:expr) (e:expr) *)
-  (* do not go in (named) depency types *)
   | LamCtxT (x:binder) (K: ectx) (f:expr) (U:expr) (e:expr)
   | LamCtxU (x:binder) (T: expr) (f:expr) (K:ectx) (e:expr)
   | LamCtx (x:binder) (T: expr) (f:expr) (U:expr) (K: ectx)
@@ -900,40 +380,9 @@ Inductive ectx :=
   | AppRCtx (e1 : expr) (K: ectx) 
   | PiCtxT (x:binder) (K: ectx) (U:expr)
   | PiCtxU (x:binder) (T:expr) (K: ectx)
-  (* (H: is_val e1) *)
-  (* only first argument in sigma *)
-  (* | SigmaCtx (x:binder) (K: ectx) (args: list (binder * expr)) *)
-    (* (H: Forall is_val es1) *)
-  (* | TupleCtx (es1:list expr) (K: ectx) (es2: list expr) 
-  (* only en is up to be a context *)
-  (* | ArrayCtx (x:binder) (K: ectx) (T:expr) *)
-  (* | PackCtx (x:binder) (K: ectx) (e:expr) *)
-  | PackLCtx (x:binder) (K: ectx) (e:expr)
-  | PackRCtx (x:binder) (en:expr) (K: ectx) 
-  | ExtractLCtx (K: ectx) (ei:expr)
- (* (H: is_val e) *)
-  | ExtractRCtx (e:expr) (K: ectx) *)
-  (*
-  TODO: nothing in types? Even toplevel
-  => array, Pi, Sigma
-  *)
   .  
 
 (* Place an expression into the hole of a context *)
-(* Fixpoint fill (K : ectx) (e : expr) : expr :=
-  match K with
-  | HoleCtx => e
-  | PiCtx x K U => Pi x (fill K e) U
-  (* | LamCtx x K f U eb => Lam x (fill K e) f U eb *)
-  | AppLCtx K v2 => App (fill K e) v2
-  | AppRCtx e1 K _ => App e1 (fill K e)
-  | SigmaCtx x K args => Sigma ((x, fill K e) :: args)
-  | TupleCtx es1 K es2 _ => Tuple (es1 ++ fill K e :: es2)
-  | ArrayCtx x K T => Array x (fill K e) T
-  | PackCtx x K eb => Pack x (fill K e) eb
-  | ExtractLCtx K ei => Extract (fill K e) ei
-  | ExtractRCtx eb K _ => Extract eb (fill K e)
-  end. *)
 Fixpoint fill (K : ectx) (e : expr) : expr :=
   match K with
   | HoleCtx => e
@@ -943,30 +392,10 @@ Fixpoint fill (K : ectx) (e : expr) : expr :=
   | PiCtxT x K U => Pi x (fill K e) U
   | PiCtxU x T K => Pi x T (fill K e)
   | AppLCtx K v2 => App (fill K e) v2
-  (* | AppRCtx e1 K H => App e1 (fill K e) *)
   | AppRCtx e1 K => App e1 (fill K e)
-  (* | TupleCtx es1 K es2 => Tuple (es1 ++ fill K e :: es2)
-  | PackLCtx x K eb => Pack x (fill K e) eb
-  | PackRCtx x en K => Pack x en (fill K e)
-  | ExtractLCtx K ei => Extract (fill K e) ei
-  | ExtractRCtx eb K => Extract eb (fill K e) *)
   end.
 
 (* Compose two evaluation contexts => place the second context into the hole of the first *)
-(* Fixpoint comp_ectx (K1: ectx) (K2 : ectx) : ectx :=
-  match K1 with
-  | HoleCtx => K2
-  | PiCtx x K U => PiCtx x (comp_ectx K K2) U
-  (* | LamCtx x K f U e => LamCtx x (comp_ectx K K2) f U e *)
-  | AppLCtx K v2 => AppLCtx (comp_ectx K K2) v2
-  | AppRCtx e1 K H => AppRCtx e1 (comp_ectx K K2) H
-  | SigmaCtx x K args => SigmaCtx x (comp_ectx K K2) args
-  | TupleCtx es1 K es2 H => TupleCtx es1 (comp_ectx K K2) es2 H
-  | ArrayCtx x K T => ArrayCtx x (comp_ectx K K2) T
-  | PackCtx x K e => PackCtx x (comp_ectx K K2) e
-  | ExtractLCtx K ei => ExtractLCtx (comp_ectx K K2) ei
-  | ExtractRCtx e K H => ExtractRCtx e (comp_ectx K K2) H
-  end. *)
 Fixpoint comp_ectx (K1: ectx) (K2 : ectx) : ectx :=
   match K1 with
   | HoleCtx => K2
@@ -976,13 +405,7 @@ Fixpoint comp_ectx (K1: ectx) (K2 : ectx) : ectx :=
   | PiCtxT x K U => PiCtxT x (comp_ectx K K2) U
   | PiCtxU x T K => PiCtxU x T (comp_ectx K K2)
   | AppLCtx K v2 => AppLCtx (comp_ectx K K2) v2
-  (* | AppRCtx e1 K H => AppRCtx e1 (comp_ectx K K2) H *)
   | AppRCtx e1 K => AppRCtx e1 (comp_ectx K K2)
-  (* | TupleCtx es1 K es2 => TupleCtx es1 (comp_ectx K K2) es2
-  | PackLCtx x K eb => PackLCtx x (comp_ectx K K2) eb
-  | PackRCtx x en K => PackRCtx x en (comp_ectx K K2)
-  | ExtractLCtx K ei => ExtractLCtx (comp_ectx K K2) ei
-  | ExtractRCtx eb K => ExtractRCtx eb (comp_ectx K K2) *)
   end.
 
 
@@ -1031,328 +454,9 @@ Proof.
   - (* Idx #n, Idx -> ... *)
     destruct K;simpl in *;inversion H1;subst.
     inversion Hred.
-    (*
-  - (* Idx #n, #n -> ... *)
-    destruct K;simpl in H2;inversion H2;subst.
-    inversion Hred.
- *)
-  (* - apply Forall_app in H0 as [H1 H2].
-    inversion H2;subst.
-    congruence. *)
 Qed.
 
 
-(*
-  assume typed and normalized
-*)
-Lemma characterize_value e:
-  ¬ reducible e → is_val e.
-Proof.
-  intros H.
-  induction e;try now econstructor.
-  (* admit. (* var -- ruled out by typed *) *)
-  - econstructor.
-    1: apply IHe1.
-    2: apply IHe2.
-    all: contradict H;destruct H as [e' [K e1' e2' -> -> Hred]].
-    all: eexists;eapply Ectx_step;eauto.
-    + now instantiate (1:=PiCtxT x K e2).
-    + now instantiate (1:=PiCtxU x e1 K).
-  - econstructor.
-    1: apply IHe1.
-    2: apply IHe3.
-    3: apply IHe4.
-    all: contradict H;destruct H as [e' [K e1' e2' -> -> Hred]].
-    all: eexists;eapply Ectx_step;eauto.
-    + now instantiate (1:=LamCtxT x K e2 e3 e4).
-    + now instantiate (1:=LamCtxU x e1 e2 K e4).
-    + now instantiate (1:=LamCtx  x e1 e2 e3 K).
-  - contradict H.
-    (* app *)
-    (* if typed and normalized => lambda => makes an app step *)
-    admit.
-  (* - admit. (* nested induction *)
-  - (* pack *)
-    admit.
-  - (* extract *)
-    (* if normalized (and typed), all extracts are evaluated *)
-    admit. *)
-Abort.
-
-
-(* TODO: we want is_val <-> ~ reducibile *)
-(* Lemma values_dont_reduce e:
-  is_val e → ¬ reducible e.
-Proof.
-  intros Hv Hred.
-  destruct Hred.
-  destruct H as [K e1 e2 -> -> Hred].
-  induction K;simpl in Hv;inversion Hv;subst;try congruence.
-  all: try (now inversion Hred).
-  - (* Idx #n, Idx -> ... *)
-    destruct K;simpl in *;inversion H0;subst.
-    inversion Hred.
-  - (* Idx #n, #n -> ... *)
-    destruct K;simpl in H2;inversion H2;subst.
-    inversion Hred.
-  - apply Forall_app in H1 as [H1 H2].
-    inversion H2;subst.
-    congruence.
-Qed. *)
-
-(*
-lemma is_val -> normalized
-equivalent: normalizable -> reducable
-
-TODO: does not hold!
-we normalize under binders but do not reduce under binders
-*)
-(* Lemma normalized_values e:
-  is_val e → normalized e.
-Proof.
-  (* could go the step over 
-    val -> ~red
-    normalizable -> reduce
-   *)
-   intros Hval [e' Hnormstep].
-   inversion Hnormstep;subst.
-   induction K;simpl in *.
-   - inversion H1;subst;admit.
-   - inversion Hval;subst.
-     apply IHK;eauto.
-     eapply Fectx_step with (K:=K);eauto.
-   - 
-
-   dependent induction Hval;simpl in *.
-   - 
-   all: inversion H1;subst.
-   - 
-
-Abort. *)
-
-(* TODO: possibly multiple steps 
-  e.g. <_:n;e>#ei ->n e
-  <_:n;e>#ei 
-    -> <_:vn;e>#ei 
-    -> <_:vn;e>#vi 
-    -> e
-
-  => use progress lemma
-
-  e#0_1 -> e
-  use canonical values => tuple/pack
-*)
-Lemma norm_red e e':
-    normalize_step e e' → base_step e e'.
-Proof.
-  intros Hnorm.
-  inversion Hnorm;subst.
-Abort.
-
-(* TODO: not necessarily: the redex might be under a binder *)
-(* Lemma normalizable_reducible e:
-  normalizable e → reducible e.
-Proof.
-  intros [e' Hnorm].
-  inversion Hnorm;subst.
-  eexists.
-  induction H1.
-Abort. *)
-
-
-
-
-
-(* Fixpoint is_closed (X : list string) (e : expr) : bool :=
-  match e with
-  | Star | Box | Bot | Nat | Idx | LitNat _ | LitIdx _ _ => true
-  | Var x => bool_decide (x ∈ X)
-  | Pi x T U => is_closed X T && is_closed (x :b: X) U
-  | Lam x T f U e => is_closed X T && is_closed (x :b: X) f && is_closed (x :b: X) U && is_closed (x :b: X) e
-  | App e1 e2 => is_closed X e1 && is_closed X e2
-  (* sigma closed under previous *)
-  | Sigma args => (fix is_closed_sigma (X : list string) (args : list (binder * expr)) : bool :=
-    match args with
-    | [] => true
-    | (x, T) :: args => is_closed X T && is_closed_sigma (x :b: X) args
-    end) X args
-  | Tuple es => forallb (is_closed X) es
-  | Array x en T => is_closed X en && is_closed (x :b: X) T
-  | Pack x en e => is_closed X en && is_closed (x :b: X) e
-  | Extract e ei => is_closed X e && is_closed X ei
-  end.
-
-(* TODO: where do we need those lemmas?
-  TODO: There are better ways to handle (or not) closedness
-*)
-
-(** [closed] states closedness as a Coq proposition, through the [Is_true] transformer. *)
-Definition closed (X : list string) (e : expr) : Prop := Is_true (is_closed X e).
-#[export] Instance closed_proof_irrel X e : ProofIrrel (closed X e).
-Proof. unfold closed. apply _. Qed.
-#[export] Instance closed_dec X e : Decision (closed X e).
-Proof. unfold closed. apply _. Defined.
-
-(** closed expressions *)
-Lemma is_closed_weaken X Y e : is_closed X e → X ⊆ Y → is_closed Y e.
-Proof. 
-  (* revert X Y; induction e; try naive_solver (eauto; set_solver).  *)
-  (* TODO: the list cases (Sigma, Tuple) => need neested induction *)
-  all: admit.
-Admitted.
-
-Lemma is_closed_weaken_nil X e : is_closed [] e → is_closed X e.
-Proof. intros. by apply is_closed_weaken with [], list_subseteq_nil. Qed.
-
-Lemma is_closed_subst X e x es :
-  is_closed [] es → is_closed (x :: X) e → is_closed X (subst x es e).
-Proof.
-  intros ?.
-  induction e in X |-*; simpl; intros ?; destruct_and?; split_and?; simplify_option_eq;
-    try match goal with
-    | H : ¬(_ ∧ _) |- _ => apply not_and_l in H as [?%dec_stable|?%dec_stable]
-    end; eauto using is_closed_weaken with set_solver.
-  (* TODO: check *)
-  all: admit.
-Admitted.
-Lemma is_closed_do_subst' X e x es :
-  is_closed [] es → is_closed (x :b: X) e → is_closed X (subst' x es e).
-Proof. destruct x; eauto using is_closed_subst. Qed.
-
-(** Substitution lemmas *)
-Lemma subst_is_closed X e x es : is_closed X e → x ∉ X → subst x es e = e.
-Proof.
-  induction e in X |-*; simpl; rewrite ?bool_decide_spec, ?andb_True; intros ??;
-    repeat case_decide; simplify_eq; simpl; f_equal; intuition eauto with set_solver.
-  (* TODO: check *)
-  all: admit.
-Admitted.
-
-Lemma subst_is_closed_nil e x es : is_closed [] e → subst x es e = e.
-Proof. intros. apply subst_is_closed with []; set_solver. Qed.
-Lemma subst'_is_closed_nil e x es : is_closed [] e → subst' x es e = e.
-Proof. intros. destruct x as [ | x]. { done. } by apply subst_is_closed_nil. Qed. *)
-
-
-
-
-
-
-
-
-
-
-
-
-
-
-
-(* we derive a few lemmas about contextual steps *)
-(*
-we need these lemmas for progress
-=> if inner expression not value, we can lift a contextual step over a context
-however, the context is an indirection over a simplification requiring a lemma to ease the automation burdon
-*)
-
-(* Lemma contextual_step_pi x T U T':
-  contextual_step T T' →
-  contextual_step (Pi x T U) (Pi x T' U).
-Proof.
-  intros Hcontextual.
-  by eapply (fill_contextual_step (PiCtx x HoleCtx U)).
-Qed.
-
-(* Lemma contextual_step_lam x ef U e T T':
-  contextual_step T T' →
-  contextual_step (Lam x T ef U e) (Lam x T' ef U e).
-Proof.
-  intros Hcontextual.
-  by eapply (fill_contextual_step (LamCtx x HoleCtx ef U e)).
-Qed. *)
-
-Lemma contextual_step_app_l e1 e1' e2:
-  contextual_step e1 e1' →
-  contextual_step (App e1 e2) (App e1' e2).
-Proof.
-  intros Hcontextual.
-  by apply (fill_contextual_step (AppLCtx HoleCtx e2)).
-Qed.
-
-Lemma contextual_step_app_r e1 e2 e2':
-  is_val e1 →
-  contextual_step e2 e2' →
-  contextual_step (App e1 e2) (App e1 e2').
-Proof.
-  intros H Hcontextual.
-  by apply (fill_contextual_step (AppRCtx e1 HoleCtx H)).
-Qed.
-
-Lemma contextual_step_sigma x T T' xs:
-  contextual_step T T' →
-  contextual_step (Sigma ((x, T) :: xs)) (Sigma ((x, T') :: xs)).
-Proof.
-  intros Hcontextual.
-  by apply (fill_contextual_step (SigmaCtx x HoleCtx xs)).
-Qed.
-
-Lemma contextual_step_tuple es es' e e':
-  Forall is_val es →
-  contextual_step e e' →
-  contextual_step (Tuple (es ++ e :: es')) (Tuple (es ++ e' :: es')).
-Proof.
-  intros Hval Hcontextual.
-  by apply (fill_contextual_step (TupleCtx es HoleCtx es' Hval)).
-Qed.
-
-Lemma contextual_step_array x en en' T:
-  contextual_step en en' →
-  contextual_step (Array x en T) (Array x en' T).
-Proof.
-  intros Hcontextual.
-  by apply (fill_contextual_step (ArrayCtx x HoleCtx T)).
-Qed.
-
-Lemma contextual_step_pack x en en' e:
-  contextual_step en en' →
-  contextual_step (Pack x en e) (Pack x en' e).
-Proof.
-  intros Hcontextual.
-  by apply (fill_contextual_step (PackCtx x HoleCtx e)).
-Qed.
-
-Lemma contextual_step_extract_l e e' ei:
-  contextual_step e e' →
-  contextual_step (Extract e ei) (Extract e' ei).
-Proof.
-  intros Hcontextual.
-  by apply (fill_contextual_step (ExtractLCtx HoleCtx ei)).
-Qed.
-
-Lemma contextual_step_extract_r e ei ei':
-  is_val e →
-  contextual_step ei ei' →
-  contextual_step (Extract e ei) (Extract e ei').
-Proof.
-  intros H Hcontextual.
-  by apply (fill_contextual_step (ExtractRCtx e HoleCtx H)).
-Qed.
-
-#[export]
-Hint Resolve
-  contextual_step_pi
-  (* contextual_step_lam *)
-  contextual_step_app_l
-  contextual_step_app_r
-  contextual_step_sigma
-  contextual_step_tuple
-  contextual_step_array
-  contextual_step_pack
-  contextual_step_extract_l
-  contextual_step_extract_r
-  : core.
-
-
- *)
 
 
  Lemma contextual_step_lambda x T f U e1 e2:
@@ -1431,11 +535,6 @@ Proof.
 Qed.
 
 
-(*
-(exists full_contextual_step) \/ normalized_pred
-because 
-normalized_pred := ~ exists full_contextual_step
-*)
 
 (*
 full_contextual_step is defined over contexts
@@ -1456,10 +555,6 @@ Proof.
       now rewrite full_fill_comp.
     + rewrite full_fill_comp.
       now apply IHrtc.
-(* Restart.
-  intros;subst.
-  eapply rtc_congruence.
-  - intros. *)
 Qed.
 
 Lemma rtc_rtc {A:Type} {R:relation A} e e' e'':
@@ -1473,37 +568,6 @@ Proof.
 Qed.
 
 
-(* Lemma normalized_dec e:
-  normalized e ∨ ¬ normalized e.
-Proof. *)
-
-
-Lemma normal_functional e:
-  {e' | normal_eval e e'}.
-Proof.
-  induction e.  
-  1-7: eexists;subst;constructor;[constructor|];apply norm_sound;constructor.
-  - destruct IHe1 as [e1' [He1' Hnorme1']].
-    destruct IHe2 as [e2' [He2' Hnorme2']].
-    exists (Pi x e1' e2').
-    constructor.
-    + eapply rtc_rtc.
-      * eapply rtc_full_contextual_context.
-        -- apply He1'.
-        -- instantiate (1:=(FPi1 x FHoleCtx e2));simpl;reflexivity.
-        -- simpl. reflexivity.
-      * eapply rtc_full_contextual_context.
-        -- apply He2'.
-        -- instantiate (1:=(FPi2 x e1' FHoleCtx));simpl;reflexivity.
-        -- simpl. reflexivity.
-    + apply norm_sound.
-      constructor;auto.
-      all: now apply norm_sound2.
-  - admit. (* same as above *)
-  - destruct IHe1 as [e1' [He1' Hnorme1']].
-    destruct IHe2 as [e2' [He2' Hnorme2']].
-    admit. (* TODO: we have the additional step *)
-Admitted.
 
 
 
