thorin/semantics/types_sol.v
@@ -3,41 +3,33 @@ From iris Require Import prelude.
 (* From thorin.lib Require Import maps. *)
 From thorin Require Import lang notation.
 Require Import Coq.Program.Equality.
+Require Import Coq.Program.Wf.
 (* From Autosubst Require Export Autosubst. *)
 
 (*
   Usually, typing uses deBrujin indices for naming
   this makes freshness, no-clash easy
+  For deBrujin indices, Autosubst provides helpful lemmas and operations
 
-  Our case is special in multiple ways:
-  - types and expressions are the same
-  - evaluation also happens in types
-  - we have multiple kind levels (the type of types has a type (at which level we get impredicative))
-  - our typing is mutual recursive with an assignability relation
-  - we have nested inductive predicates
+  Our system is very similar to the calculus of construction
+  as presented, for instance, in "Typed Lambda Calculus / Calculus of
+Constructions" by Brandl
+  (https://hbr.github.io/Lambda-Calculus/cc-tex/cc.pdf)
 
-  Autosubst has support for De Bruijn indices and their substitution
-  Usually, the typing is annotated with the type level in the presence of indices
-  and lifting lemmas are defined
+  Our additions lie in the zip calculus (not discussed here for brevity),
+  axioms (handled at this stage), and normalization.
 
+  Our reduction goes under binder and evaluation also happens on type level.
 
-  The most important difference to CC is that we have no rule that types can be beta equivalent
-  for typing.
-  Additionally, we have normalization operations that are applied eagerly at every construction
+  The most important difference to CC is that we have no rule that types can be beta equivalent for typing.
+  Although we add such a rule for preservation (see below).
+  Our normalization operations are applied eagerly at every construction and can be assumed as precondition for every expression.
 *)
-
-
 
 Definition typing_context := gmap string expr.
 Implicit Types
   (Γ : typing_context)
   (e : expr).
-
-
-(* TODO: check with page 46 in https://hbr.github.io/Lambda-Calculus/cc-tex/cc.pdf *)
-
-Require Import Coq.Program.Wf.
-
 
 Definition Star := Sort 0.
 Definition insert_name (x: binder) (e: expr) (Γ: typing_context) :=
@@ -46,14 +38,7 @@ Definition insert_name (x: binder) (e: expr) (Γ: typing_context) :=
   | BAnon => Γ
   end.
 
-(*
-We left out zip calculus
-and axioms
-Without the zip calculus, type assignability becomes normal typing
-
-instead of named and unnamed variants, we use insert_name to unify both into one
-*)
-
+(* instead of named and unnamed variants (as is common), we use insert_name to unify both into one *)
 Reserved Notation "'TY' Γ ⊢ e : A" (at level 74, e, A at next level).
 Reserved Notation "'TY' Γ ⊢ A ← e" (at level 74, e, A at next level).
 Inductive syn_typed : typing_context → expr → expr → Prop :=
@@ -101,20 +86,6 @@ where "'TY' Γ ⊢ e : A" := (syn_typed Γ e%E A%E)
 .
 #[export] Hint Constructors syn_typed : core.
 
-Lemma typed_weakening Γ Δ e A:
-  TY Γ ⊢ e : A →
-  Γ ⊆ Δ →
-  TY Δ ⊢ e : A.
-Proof.
-  intros HTy Hsub.
-  induction HTy;eauto.
-Admitted.
-
-
-
-
-
-
 (*
 Specialization to subst for fmap_insert since Coq won't recognize (subst a e') as function application point
 *)
@@ -133,23 +104,12 @@ Qed.
 (*
   Substitution reordering to distrubte the subst from typing predicates to the outside
   for induction hypotheses
+
+  We assume lemmas about renaming/name clash avoidance
 *)
-Lemma subst_distr x a e1 e2 e3:
+Axiom (subst_distr: forall x a e1 e2 e3,
   a ≠ x →
-  subst a e1 (subst x e2 e3) = subst x (subst a e1 e2) (subst a e1 e3).
-Proof.
-  intros Hneq.
-  induction e3;simpl;try congruence.
-  - destruct (decide) as [Heq|Heq];simpl.
-    + rewrite Heq. 
-      destruct decide;try congruence.
-      simpl.
-      now destruct decide;congruence.
-    + destruct decide as [Heq'|Heq'].
-      * admit. 
-      * simpl. destruct decide;congruence.
-  (* ... *)
-Admitted.
+  subst a e1 (subst x e2 e3) = subst x (subst a e1 e2) (subst a e1 e3)).
 
 Corollary subst'_distr x a e1 e2 e3:
   BNamed a ≠ x →
@@ -162,278 +122,17 @@ Proof.
     contradict H. congruence.
 Qed.
 
-
 (*
-Substitution lemmas
-|- e' : A
-Γ, x : A ⊢ e : B
-=================
-Γ ⊢ e[e'/x] : B[e'/x]
+One of our main lemmas:
+Well typed expressions are not stuck
+=> either step or are values
 
-Note: Importantly, we need to substitute in the type as well as it might contain/depend on the variable x.
-
-Also see page 55 in
-https://hbr.github.io/Lambda-Calculus/cc-tex/cc.pdf
-*)
-Lemma typed_substitutivity e e' Γ (a: binder) A B 
-  Γ' e'_norm B'_norm:
-  (* TY ∅ ⊢ e' : A → *)
-  TY Γ ⊢ e' : A →
-  TY (insert_name a A Γ) ⊢ e : B →
-  normal_eval (lang.subst' a e' e) e'_norm →
-  normal_eval (lang.subst' a e' B) B'_norm →
-  (forall x v,
-    Γ !! x = Some v <-> (exists k, Γ' !! x = Some k /\ normal_eval (subst' a e' v) k)) ->
-    (* /\ Γ' !! x = Some v -> (exists k, Γ' !! x = Some k /\ normal_eval (subst' a e' v) k) -> *)
-  TY Γ' ⊢ e'_norm : B'_norm.
-Proof.
-  assert (lang.subst' a e' A = A) as HsubstA by admit.
-  intros He' H Hnorme HnormB HΓ.
-  (* 
-  induction e + inversion lemmas alone are not enough due to dependencies
-  subst B : ... is missing => needs hypothesis 
-  *)
-  revert Γ' e'_norm B'_norm Hnorme HnormB HΓ.
-  dependent induction H;simpl;eauto.
-  all: intros Γ' e'_norm B'_norm Hnorme HnormB HΓ.
-  - (* Sort *)
-    replace e'_norm with (Sort n) by admit.
-    replace B'_norm with (Sort (S n)) by admit.
-    econstructor.
-  - (* Bot *)
-    replace e'_norm with Bot by admit.
-    replace B'_norm with Star by admit.
-    econstructor.
-  - (* Nat *)
-    replace e'_norm with Nat by admit.
-    replace B'_norm with Star by admit.
-    econstructor.
-  - (* Idx *)
-    replace e'_norm with Idx by admit.
-    replace B'_norm with (Pi BAnon Nat Star) by admit.
-    econstructor.
-  - (* LitNat *)
-    replace e'_norm with (#n)%E by admit.
-    replace B'_norm with Nat by admit.
-    econstructor.
-  - (* LitIdx *)
-    replace e'_norm with (LitIdx n i) by admit.
-    replace B'_norm with (App Idx n) by admit.
-    econstructor.
-  - (* Var *)
-    replace e'_norm with (Var x) by admit.
-    (* needs Environment normalized *)
-    econstructor.
-    admit. (* relate Γ and Γ' *)
-  - (* Pi *)
-    replace (subst' a e' (Pi x T U)) with (Pi x (subst' a e' T) (subst' a e' U)) in Hnorme by admit.
-    (* destruct decide in Hnorme;[admit|]. *)
-    assert(
-      exists T' U',
-      e'_norm = Pi x T' U' /\
-      normal_eval (subst' a e' T) T' /\
-      normal_eval (subst' a e' U) U'
-    ) as [T' [U' [He'_norm [HnormT HnormU]]]] by admit.
-    subst.
-    simpl in HnormB.
-    replace (B'_norm) with (LitNat(max sT sU)) by admit.
-    econstructor.
-    + eapply IHsyn_typed1.
-      4: eapply HnormT.
-      4: admit. (* Sort norm *)
-      2: eassumption.
-      1: eassumption.
-      reflexivity.
-      eassumption.
-    + eapply IHsyn_typed2.
-      4: eassumption.
-      4: admit. (* Sort norm *)
-      1-2: eassumption.
-      admit. (* different order insert *)
-      (* eassumption. *)
-      admit. (* Γ' *)
-  - (* Lambda *)
-    replace (subst' a e' (Lam x T ef U e)) with (Lam x (subst' a e' T) (subst' a e' ef) (subst' a e' U) (subst' a e' e)) in Hnorme by admit.
-    pose proof HnormB as HnormB2.
-    replace (subst' a e' (Pi x T U)) with (Pi x (subst' a e' T) (subst' a e' U)) in HnormB2 by admit.
-    assert(
-      exists T' U' ef' e'',
-      e'_norm = Lam x T' ef' U' e'' /\
-      normal_eval (subst' a e' T) T' /\
-      normal_eval (subst' a e' ef) ef' /\
-      normal_eval (subst' a e' U) U'
-    ) as [T' [U' [ef' [e'' [He'_norm [HnormT [Hnormef HnormU]]]]]]] by admit.
-    subst.
-    assert(
-      exists T'' U'',
-      B'_norm = Pi x T'' U'' /\
-      normal_eval (subst' a e' T) T'' /\
-      normal_eval (subst' a e' U) U''
-    ) as [T'' [U'' [HB'_norm [HnormT' HnormU']]]] by admit.
-    subst.
-    (* confluence of normalize *)
-    assert (T' = T'') as -> by admit.
-    assert (U' = U'') as -> by admit. 
-    econstructor.
-    + eapply IHsyn_typed1.
-      2-6: try eassumption.
-      1-2: eauto.
-      all: admit. (* TODO: subst in sort *)
-      (* 4: eapply HnormB.
-      3: reflexivity.
-      1-2: eassumption.
-      admit. (* TODO: where does s come from *)
-      eassumption. *)
-    + eapply IHsyn_typed2.
-      4: eassumption.
-      1-2: eassumption.
-      1: admit. (* insert order *)
-      admit. (* bool norm bool *)
-      admit. (* Γ' *)
-    + admit. (* TODO: assignability induction *)
-    + admit. (* TODO: *)
-  - (* App *)
-    admit. (* TODO *)
-Admitted.
-
-
-
-
-
-(*
-canonical values (see one from above for Idx)
-(specific type, rest generic, and is value expression)
-
-  e : Idx #n 
-e : Idx en (unnecessary?)
-  e : Array x en T (changes under normalization lemma)
-  e : Sigma Ts
-  e : Pi x T U
-  e : Nat
-*)
-(* all general cases that are contradictory 
-  manually identified while proving the canonical value idx lemma
-*)
-Ltac no_nonsense_canonical := 
-  first 
-  [
-    (*
-      Look for assumption sort (...) where the inner is not Star or Box
-      try to apply inversion;congruence
-
-      Array named/anon
-    *)
-    (* match goal with
-    | H: sort ?s |- _ => try (inversion H;congruence)
-    end
-  | *)
-    (*
-      Look for assumption kind_dominance xs s where s is not Star, Box or a variable
-      apply canonical_kind;congruence
-
-      Pi named/anon, Sigma named/anon
-    *)
-    (* match goal with
-    | H: kind_dominance ?xs ?s |- _ => try (apply canonical_kind in H as [];congruence)
-    end
-  | *)
-    (* 
-    find an illegal Idx expression as function value
-    e.g.
-    H0: TY Γ ⊢ Idx : Pi x T U
-    H: subst' x #n U = X
-    where X is not star
-    => we need to find two assumptions that contradict
-
-    Idx #n as value via App case
-    *)
-      (* idtac "found1"; *)
-    match goal with
-    | H0: (TY ?Γ ⊢ Idx : Pi ?x ?T ?U),
-      H: (subst' ?x ?e ?U = ?X)
-      |- _ => 
-      (* idtac "found" *)
-      try (inversion H0;subst;simpl in H;congruence)
-    end
-  ].
-
-
-
-(* is it sufficient to have n fixed as a nat or do we want more generally ⊢ en : Nat *)
-Lemma canonical_value_idx Γ e (n:nat):
-  TY Γ ⊢ e : Idx (LitNat n) ->
-  is_val e ->
-  exists i, e = LitIdx n i.
-Proof.
-  intros Hty Hv.
-  inversion Hty;subst;try naive_solver;inversion Hv;subst;try no_nonsense_canonical.
-  inversion H;subst.
-  simpl in H1.
-  admit. (* Star does not normalize to Idx *)
-Admitted.
-
-
-Lemma canonical_value_pi Γ e x T U:
-  TY Γ ⊢ e : Pi x T U →
-  is_val e ->
-  
-  (e = Idx ∧ x = BAnon /\ T = Nat ∧ U = Star) ∨
-  exists f ef, 
-    (e = Lam x T f U ef).
-Proof.
-  intros Hty Hv.
-  inversion Hty;subst;try naive_solver;inversion Hv;subst;try no_nonsense_canonical.
-  inversion H;subst.
-  admit. (* Star does not normalize to Pi *)
-Admitted.
-
-Lemma canonical_value_nat Γ e:
-  TY Γ ⊢ e : Nat →
-  is_val e ->
-  
-  exists n, e = LitNat n.
-Proof.
-  intros Hty Hv.
-  inversion Hty;subst;try naive_solver;inversion Hv;subst; try no_nonsense_canonical.
-  inversion H;subst.
-  admit. (* Star does not normalize to Nat *)
-Admitted.
-
-
-
-
-
-
-
-
-
-
-(*
 Progress 
 |- e : A
 =================
 e is a value or
 exists e' s.t. e -> e'
 *)
-(*
-  TODO: need empty env => variable is not a value and not reducible
-*)
-(*
-but this does not work for U in Pi, for instance, we need a different env
-=> reduction under binder
-Corollary typed_progress e A:
-  TY ∅ ⊢ e : A →
-  is_val e ∨ reducible e.
-Proof.
-  intros HTy.
-  remember ∅ as Γ eqn:HΓ.
-  induction HTy.
-  all: subst;eauto 10 using is_val.
-  - admit. (* in empty env, we would not have var *)
-  - (* Pi *)
-*)
-
-
 Corollary typed_progress Γ e A:
   TY Γ ⊢ e : A →
   is_val e ∨ reducible e.
@@ -441,34 +140,31 @@ Proof.
   intros HTy.
   induction HTy.
   all: subst;eauto 10 using is_val.
-  - admit. (* in empty env, we would not have var *)
-  (* 
   - (* Pi *)
-    destruct IHHTy1 as [HvalT|[? ?]].
-    + destruct IHHTy2 as [HvalU|[? ?]].
-      (* * destruct IHHTy4 as [Hvale|[? ?]];[|right;eexists;eauto].
-        left. 
-        now constructor. *)
-      * right. eexists. eauto.
-    + right. eexists. eauto.
-    *)
+    destruct IHHTy1 as [HvalT|[? ?]];[|right;eexists;eauto].
+    destruct IHHTy2 as [HvalU|[? ?]];[|right;eexists;eauto].
+    left. now constructor.
   - (* Lambda *)
     destruct IHHTy4 as [Hvale|[? ?]];[|right;eexists;eauto].
     destruct IHHTy2 as [HvalU|[? ?]];[|right;eexists;eauto].
     destruct IHHTy1 as [HvalT|[? ?]];[|right;eexists;eauto].
-    left. 
-    now constructor.
+    left. now constructor.
   - (* App *)
     (* only value for Idx n *)
     destruct IHHTy1 as [Hvale|[? ?]];[|right;eexists;eauto].
     destruct IHHTy2 as [Hvale2|[? ?]];[|right;eexists;eauto].
-    specialize (canonical_value_pi _ _ _ _ _ HTy1 Hvale) as [(->&->&->&->)|(f&ef&->)].
-    + (* Idx *)
-      specialize (canonical_value_nat _ _ HTy2 Hvale2) as [m ->].
-      left. constructor.
-    + right. eexists. eapply base_contextual_step.
-      eapply BetaS. reflexivity.
-Admitted.
+
+    (*
+    usually, we would have canonical values for Pi => lam or Idx: Nat -> Star
+    and Nat => Lit
+    Here, our application are more general (all non-redexes due to variables)
+    *)
+    destruct e.
+    all: try now (left;constructor;eauto).
+    right. eexists. 
+    eapply base_contextual_step.
+    eapply BetaS. reflexivity.
+Qed.
 
 
 Lemma Forall2_nth_error {X Y:Type} (P: X -> Y -> Prop) xs ys:
@@ -501,7 +197,6 @@ Furthermore, the change of typed in argument position breaks type dependencies.
 Hence, one beta step is not enough.
 Therefore, only eventually (after multiple step), a consistent (typed) state is reached.
 
-
 Γ ⊢ e : A
 e →β e'
 =================
@@ -510,31 +205,14 @@ e' →*β e'' →n e'''
 A  →*β A'  →n A''
 Γ ⊢ e''' : A''
 
+Instead, we allow for the usual beta equivalence in types.
+
+This way, our typing embeds: Every typed expression is also typed in "normal CC"
+Then, a step preserves typing (modulo beta equivalence)
+Hence, we end in a beta-equivalent type
+For thorin's type fragment (e.g. finite termination on type level), the embed back works by normalization/furhter steps.
+
 *)
-
-(*
-stronger than (probably necessary) but provable
-
-Note base_step is only toplevel (→ᵦ is also contextual)
-*)
-Lemma typed_preservation_base_step e e' Γ A
-  e'_norm:
-  TY Γ ⊢ e : A →
-  base_step e e' →
-  normal_eval e' e'_norm →
-  TY Γ ⊢ e'_norm : A.
-Proof.
-  intros Hty Hstep Hnorm.
-  inversion Hstep;subst.
-  inversion Hty;subst;eauto using is_val.
-  inversion H1;subst.
-
-  eapply typed_substitutivity.
-  3-4: eassumption.
-  2: eassumption.
-  1: eassumption.
-  admit. (* simple *)
-Admitted.
 
 Lemma fill_step K e1 e2:
   base_step e1 e2 ->
@@ -560,12 +238,10 @@ Qed.
 
 
 (*
-just symmetry, refl, trans +
-(lam A. B) C = B [x := C]
-
-or via beta
+just symmetry, refl, trans + (lam A. B) C = B [x := C]
+or via beta reduction closure
 *)
-Definition equiv (A B:expr) := True.
+Definition equiv (A B:expr) := exists C, A →ᵦₙ* C ∧ B →ᵦₙ* C.
 Notation "A ≡ᵦ B" := (equiv A B) (at level 70).
 
 
@@ -769,8 +445,6 @@ Proof.
         split;eauto.
 Qed.
 
-
-
 Lemma normalized_norm_eval e e':
   normalized e →
   e →ₙ e' →
@@ -794,7 +468,7 @@ Proof.
   intros H1 H2.
   destruct H1 as [Hstep1 Hnorm1%norm_sound2].
   destruct H2 as [Hstep2 Hnorm2%norm_sound2].
-  admit.
+  admit. (* TODO: 2 *)
 Admitted.
 
 
@@ -874,7 +548,7 @@ Proof.
     + rewrite lookup_insert in Hk.
       rewrite lookup_insert.
       (* inversion Hk;subst. *)
-      admit.
+      admit. (* TODO: 2 *)
     + rewrite lookup_insert_ne in Hk;eauto.
       rewrite lookup_insert_ne;eauto.
 Admitted.
@@ -907,31 +581,6 @@ Proof.
     all: econstructor;eauto;econstructor;eauto.
 Qed.
 
-
-(* Lemma pi_norm x T U e'_norm:
-  Pi x T U →ₙ e'_norm ->
-      exists T'' U'',
-      e'_norm = Pi x T'' U'' /\
-      normal_eval T T'' /\
-      normal_eval U U''.
-Proof.
-  intros [Hstep Hnorm%norm_sound2].
-  dependent induction Hstep.
-  - inversion Hnorm;subst.
-    do 2 eexists. 
-    firstorder.
-    1,3: reflexivity.
-    all: now apply norm_sound.
-  - inversion H;subst.
-    destruct K;simpl in *;inversion H0;subst.
-    1: {inversion H2. }
-    1: specialize (IHHstep x0 (full_fill K e2') U0).
-    2: specialize (IHHstep x0 K (full_fill K0 e2')).
-    all: destruct IHHstep as (T'&U'&->&[HTs HTn]&[HUs HUn]);eauto.
-    all: do 2 eexists;firstorder.
-    all: econstructor;eauto;econstructor;eauto.
-Qed. *)
-
 Lemma subst'_bot a e:
   subst' a e Bot = Bot.
 Proof.
@@ -947,6 +596,95 @@ Proof.
 Qed.
 
 
+Lemma norm_beta_preserve A B A' B':
+  A ≡ᵦ B ->
+  A →ₙ A' ->
+  B →ₙ B' ->
+  A' ≡ᵦ B'.
+Proof.
+  (* intros [C [[AC [Hb1 Hn1]] [BC [Hb2 Hn2]]]] H3 H4. *)
+  (* add norm to front *)
+  (* TODO: 2 *)
+Admitted.
+
+
+Lemma normal_functional e:
+  {e' | normal_eval e e'}.
+Proof.
+  induction e.  
+  1-7: eexists;subst;constructor;[constructor|];apply norm_sound;constructor.
+  - destruct IHe1 as [e1' [He1' Hnorme1']].
+    destruct IHe2 as [e2' [He2' Hnorme2']].
+    exists (Pi x e1' e2').
+    constructor.
+    + eapply rtc_rtc.
+      * eapply rtc_full_contextual_context.
+        -- apply He1'.
+        -- instantiate (1:=(FPi1 x FHoleCtx e2));simpl;reflexivity.
+        -- simpl. reflexivity.
+      * eapply rtc_full_contextual_context.
+        -- apply He2'.
+        -- instantiate (1:=(FPi2 x e1' FHoleCtx));simpl;reflexivity.
+        -- simpl. reflexivity.
+    + apply norm_sound.
+      constructor;auto.
+      all: now apply norm_sound2.
+  - destruct IHe1 as [e1' [He1' Hnorme1']].
+    destruct IHe2 as [e2' [He2' Hnorme2']].
+    destruct IHe3 as [e3' [He3' Hnorme3']].
+    destruct IHe4 as [e4' [He4' Hnorme4']].
+    exists (Lam x e1' e2' e3' e4').
+    constructor.
+    + eapply rtc_rtc.
+      1: eapply rtc_full_contextual_context with (K:=FLam1 x FHoleCtx e2 e3 e4);[apply He1'| |];simpl;reflexivity.
+      eapply rtc_rtc.
+      1: eapply rtc_full_contextual_context with (K:=FLam2 x e1' FHoleCtx e3 e4);[apply He2'| |];simpl;reflexivity.
+      eapply rtc_rtc.
+      1: eapply rtc_full_contextual_context with (K:=FLam3 x e1' e2' FHoleCtx e4);[apply He3'| |];simpl;reflexivity.
+      eapply rtc_rtc.
+      1: eapply rtc_full_contextual_context with (K:=FLam4 x e1' e2' e3' FHoleCtx);[apply He4'| |];simpl;reflexivity.
+      constructor.
+    + apply norm_sound.
+      constructor;auto.
+      all: now apply norm_sound2.
+  - destruct IHe1 as [e1' [He1' Hnorme1']].
+    destruct IHe2 as [e2' [He2' Hnorme2']].
+    assert(rtc full_contextual_step (App e1 e2) (App e1' e2')).
+    {
+      eapply rtc_rtc.
+      1: eapply rtc_full_contextual_context with (K:=FApp1 FHoleCtx e2);[apply He1'| |];simpl;reflexivity.
+      eapply rtc_rtc.
+      1: eapply rtc_full_contextual_context with (K:=FApp2 e1' FHoleCtx);[apply He2'| |];simpl;reflexivity.
+      constructor.
+    }
+    (* assert(
+      (* (exists x T ef U eb, e1' = Lam x T ef U eb) \/ *)
+      {x & {T & {ef & {U & {eb & e1' = Lam x T ef U eb}}}}} +
+      (forall x T ef U eb, e1' ≠ Lam x T ef U eb)
+      (* ~is_lam *)
+    ) as [(?&?&?&?&?&->)|?].
+    {
+      admit.
+    }
+    Print full_contextual_step.
+    Print normalize_step. *)
+    admit. (* TODO: we have the additional step *)
+    (* TODO: 2 *)
+Admitted.
+
+
+Lemma subst_expression_norm_type Γ x e' A Γ' e'_norm B'_norm:
+  TY Γ ⊢ᵦ e' : A ->
+  e' →ₙ e'_norm ->
+  subst x e' A →ₙ B'_norm ->
+  gamma_relation Γ Γ' (λ v k : expr, subst x e' v →ₙ k) ->
+  TY Γ' ⊢ᵦ e'_norm : B'_norm.
+Proof.
+  assert (subst x e' A = A) as HsubstA by admit. (* avoid name clash *)
+  rewrite HsubstA.
+Admitted.
+
+(* TODO: 2 *)
 Lemma beta_typed_substitutivity e e' Γ (a: binder) A B 
   Γ' e'_norm B'_norm:
   TY Γ ⊢ᵦ e' : A →
@@ -955,11 +693,10 @@ Lemma beta_typed_substitutivity e e' Γ (a: binder) A B
   normal_eval (lang.subst' a e' B) B'_norm →
   (* (forall x v,
     Γ !! x = Some v <-> (exists k, Γ' !! x = Some k /\ normal_eval (subst' a e' v) k)) -> *)
-  gamma_relation Γ Γ' (fun v k => normal_eval (subst' a e' v) k) ->
     (* /\ Γ' !! x = Some v -> (exists k, Γ' !! x = Some k /\ normal_eval (subst' a e' v) k) -> *)
+  gamma_relation Γ Γ' (fun v k => normal_eval (subst' a e' v) k) ->
   TY Γ' ⊢ᵦ e'_norm : B'_norm.
 Proof.
-  assert (lang.subst' a e' A = A) as HsubstA by admit.
   intros He' H Hnorme HnormB HΓ.
   (* 
   induction e + inversion lemmas alone are not enough due to dependencies
@@ -1058,8 +795,7 @@ Proof.
       (* This is: replace A0 with A in *. *)
       rewrite lookup_insert in H.
       inversion H;subst.
-      rewrite HsubstA in HnormB.
-      admit. (* TODO: if typed, both normalized => still typed *)
+      eapply subst_expression_norm_type;eauto.
     + replace (subst' y e' x) with (Var x) in Hnorme by (simpl;destruct decide;congruence).
       replace e'_norm with (Var x).
       2: now apply normalized_norm_eval in Hnorme;[|econstructor].
@@ -1095,16 +831,14 @@ Proof.
     }
     econstructor.
     + eapply IHbeta_syn_typed1.
-      4: eapply HnormT.
-      4: rewrite sort_subst_inv;now apply sort_norm.
-      2: eassumption.
+      3: eapply HnormT.
+      3: rewrite sort_subst_inv;now apply sort_norm.
       1: eassumption.
       reflexivity.
       eassumption.
     + eapply IHbeta_syn_typed2 with (Γ := insert_name x T Γ).
-      4: eassumption.
-      4: rewrite sort_subst_inv;now apply sort_norm.
-      1: eassumption.
+      3: eassumption.
+      3: rewrite sort_subst_inv;now apply sort_norm.
       1: admit. (* x not free in e' => no overlap *)
       1: admit. (* different order insert *)
       apply Gamma_insert_property;eauto.
@@ -1144,13 +878,12 @@ Proof.
     assert (U' = U'') as -> by admit. 
     econstructor.
     + eapply IHbeta_syn_typed1.
-      2-6: try eassumption.
+      2-5: try eassumption.
       1-2: eauto.
       replace (subst' a e' (Sort sT)) with (Sort sT) by now destruct a.
       constructor;[constructor|apply norm_sound;constructor].
     + eapply IHbeta_syn_typed2 with (Γ := insert_name x T Γ).
-      4: eassumption.
-      1: eassumption.
+      3: eassumption.
       1: admit. (* no overlap *)
       1: admit. (* insert order *)
       1: {
@@ -1180,8 +913,9 @@ Proof.
     + eapply beta_typed_app.
       * eapply IHbeta_syn_typed1;eauto. admit. (* type norm *)
       * eapply IHbeta_syn_typed2;eauto. admit. (* type norm *)
-      * admit.
-    + admit. (* TODO: *)
+      * admit. (* e2' instead of e' in subst *)
+    + specialize (IHbeta_syn_typed1 _ _ _ He' eq_refl).
+      admit. (* TODO: *)
     (*
     assert(
       exists se' seT',
@@ -1198,7 +932,38 @@ Proof.
     (* assert (TY insert_name a A Γ ⊢ᵦ e : B) as Hty by admit.
     clear H.
     eapply IHbeta_syn_typed;eauto. *)
-  admit.
+    specialize (IHbeta_syn_typed Γ a A He' eq_refl).
+
+    (*
+    generalize over A0?
+    allow for more beta equiv?
+    convert type of e by rule?
+      => we have e: B (not needed)
+      => we need subst A0 -> B'_norm (does not hold (only beta equiv))
+    convert goal by conv rule?
+      we have e'_norm : A0_subst_norm 
+      => need A0_subst_norm equiv B'_norm
+    *)
+    assert(exists A0',
+      subst' a e' A0 →ₙ A0'
+    ) as [A0' HnormA0].
+    {
+      edestruct normal_functional.
+      eexists. eauto.
+    }
+    assert (A0' ≡ᵦ B'_norm) as Hconv.
+    {
+      eapply norm_beta_preserve.
+      2, 3: eassumption.
+      (*
+        if A0 equiv B
+        then 
+        subst a e' A0 equiv subst a e' B
+      *)
+      admit.
+    }
+    eapply beta_typed_conv;[|eassumption].
+    eapply IHbeta_syn_typed;eauto.
 Admitted.
 
 
@@ -1217,17 +982,6 @@ Proof.
   revert e2 Hstep e' Hnorm.
   dependent induction HTy;intros e2 Hstep e' Hnorm;cbn in *.
   all: try now (destruct K;cbn in *;inversion x;subst;inversion Hstep).
-  (* 
-  - admit. (* Sort *)
-  - admit. (* Bot *)
-  - (* Nat *)
-    destruct K;cbn in *;inversion x;subst;inversion Hstep.
-  - admit. (* Idx *)
-  - admit. (* LitNat *)
-  - admit. (* LitIdx *)
-  - admit. (* Var *)
-  *)
-
   - (* Pi *)
     destruct K;cbn in *;inversion x;subst.
     + inversion Hstep.
@@ -1240,7 +994,7 @@ Proof.
       eapply beta_typed_pi.
       * eapply IHHTy1;eauto.
       * (* step in context *)
-        admit.
+        admit. (* TODO: 2 *)
     + (* step in codom *)
       assert (
         exists Ke2',
@@ -1315,10 +1069,9 @@ Proof.
       rename eb into elam.
 
       (* inversion Hstep';subst. *)
-      pose proof typed_substitutivity.
+      pose proof beta_typed_substitutivity.
       specialize (H0 elam v2 Γ x1).
       specialize (H0 T).
-      replace (syn_typed) with beta_syn_typed in H0 by admit.
       assert(TY (insert_name x1 T Γ) ⊢ᵦ elam : U0) as Htyelam by admit.
       (* assert (x=x0) as ->.  {
         inversion HTy1;eauto.
@@ -1361,11 +1114,9 @@ Proof.
     (* simpl in *.
     subst. *)
     inversion Hstep;subst.
-    Check typed_substitutivity.
-    pose proof typed_substitutivity.
+    pose proof beta_typed_substitutivity.
     specialize (H1 elam eT Γ x).
     specialize (H1 T).
-    replace (syn_typed) with beta_syn_typed in H1 by admit.
     (* assert(exists B',
       TY (insert_name x T Γ) ⊢ᵦ elam : B'
     ) as [B' Htyelam] by admit. *)
@@ -1467,846 +1218,3 @@ Admitted.
 
 
 
-
-
-
-Definition equivalent e1 e2 :=
-  exists e', e1 →ᵦₙ* e' ∧ e2 →ᵦₙ* e'.
-
-Notation "e1 ≡ e2" := (equivalent e1 e2) (at level 70).
-
-(*
-if two expressions are typed and equivalent
-then their types are equivalent
-*)
-Lemma equivalent_types e1 e2 A1 A2 Γ:
-  TY Γ ⊢ e1 : A1 →
-  TY Γ ⊢ e2 : A2 →
-  e1 ≡ e2 →
-  A1 ≡ A2.
-Proof.
-  intros HTy1 HTy2 Heq.
-  destruct Heq as [e' [H1 H2]].
-  induction H1 in e2,H2,HTy1,HTy2 |-*.
-  - admit. (* base step *)
-  - admit. (* transitivity *)
-
-  (*
-  
-  could go e1 last step to e'
-  now back what is intermediate
-
-  e' does not necessarily need to be typed
-  *)
-
-
-
-
-
-
-(* 
-like beta but annotated with evaluation point 
-for partial application, we want ep as first argument
-however, from the type point, ep is a non-uniform parameter
-*)
-Inductive graded_contextual_step (ep:expr) (e1 : expr) (e2 : expr) : Prop :=
-  Ectx_step K e1' e2' :
-    e1 = fill K e1' → e2 = fill K e2' →
-    ep = e1' →
-    base_step e1' e2' → graded_contextual_step ep e1 e2.
-
-Notation "e →[ ep ]ᵦ e'" := (graded_contextual_step ep e e') (at level 50).
-Notation "e →[ ep ]ᵦ* e'" := (rtc (graded_contextual_step ep) e e') (at level 50).
-
-Definition beta_normal_step ep e e' :=
-  exists e_aux, e →[ep]ᵦ e_aux /\ e_aux →ₙ e'.
-
-Notation "e →[ ep ]ᵦₙ e'" := (beta_normal_step ep e e') (at level 50).
-Notation "e →[ ep ]ᵦₙ* e'" := (rtc (beta_normal_step ep) e e') (at level 50).
-
-
-
-(*
-Idea: dependencies can only be between lambda and its argument
-=> if doing a step with ep, we need to do more of them to reach a stable state
-
-Similarly, our type change is caused by a reduction, hence the change is the same as this reduction
-*)
-
-Definition all_beta_steps b e e' :=
-  e →[b]ᵦₙ* e' /\ ~ exists e'', e' →[b]ᵦ e''.
-
-Notation "e →|[ ep ] e'" := (all_beta_steps ep e e') (at level 50).
-
-(*
-single or uncoordinated parallel steps are not enough
-for typing, we need special steps
-
-=> we need to do all (maybe direct not recursive) "special" steps 
-
-TODO: can be do all steps instead?
-
-*)
-
-
-
-Lemma typed_preservation_eventually
-  Γ e A:
-  TY Γ ⊢ e : A →
-  forall e' A' b,
-  e →|[b] e' →
-  A →|[b] A' →
-  TY Γ ⊢ e' : A'.
-Proof.
-  intros HTy. 
-  pose proof (HTyCpy := HTy).
-  induction HTy.
-  (* do not step *)
-  1,2,3,4,5,6,7: admit.
-  (* only Pi, Lam, App left *)
-  all: intros e' A' b Hstepe HstepA.
-  - (* Pi *)
-    assert (
-      exists T' U',
-      e' = Pi x T' U' /\ 
-      T →|[b] T' /\
-      U →|[b] U'
-    ) as (T'&U'&->&HT&HU) by admit.
-    assert (A' = LitNat(sT `max` sU)) as -> by admit.
-    apply typed_pi.
-    + eapply IHHTy1;eauto.
-      admit. (* Sort -> Sort *)
-    + replace (T') with T by admit. (* step in env *)
-      eapply IHHTy2;eauto.
-      admit. (* Sort -> Sort *)
-  - (* Lam *)
-    rename e into eB.
-    assert(
-      exists T' ef' U' eB',
-      T →|[b] T' /\
-      U →|[b] U' /\
-      ef →|[b] ef' /\
-      eB →|[b] eB' /\
-      e' = Lam x T' ef' U' eB'
-    ) as (
-      T'&ef'&U'&eB'&
-      HT&HU&Hef&HeB&->
-    ) by admit.
-
-    assert (
-      exists T'' U'',
-      A' = Pi x T'' U'' /\ 
-      T →|[b] T'' /\
-      U →|[b] U''
-    ) as (T''&U''&->&HT2&HU2) by admit.
-
-    replace T'' with T' by admit. (* Deterministic →| *)
-    replace U'' with U' by admit. (* Deterministic →| *)
-    econstructor.
-    1: {
-      eapply IHHTy1;eauto.
-      admit. (* Sort -> Sort *)
-    }
-    all: replace T' with T by admit. (* step in env *)
-    + eapply IHHTy2;eauto. admit. (* Sort -> Sort *)
-    + eapply IHHTy3;eauto. admit. (* Bool -> Bool *)
-    + eapply IHHTy4;eauto.
-
-
-  - (* App *)
-    rename e into eL.
-    rename U' into sU.
-    rename A' into sU'.
-
-    (* simplified case *)
-    assert(
-      exists eL' eT',
-      eL →|[b] eL' /\
-      eT →|[b] eT' /\
-      e' = eL' eT'
-    ) as (eL'&eT'&HeL&HeT&->) by admit.
-
-    assert (
-      exists T' U',
-      Pi x T U →|[b] Pi x T' U' /\
-      T →|[b] T' /\
-      U →|[b] U'
-    ) as (T'&U'&HPi&HT&HU) by admit.
-
-    econstructor.
-    1: {
-      eapply IHHTy1;eauto.
-    }
-    1: {
-      eapply IHHTy2;eauto.
-    }
-
-
-    (*
-      here is an important difference to general beta
-      (or eval to value directly):
-      - 
-
-      U[eT/x] ->n sU
-      sU ->| sU'
-      U ->| U'
-      eT ->| eT'
-
-
-
-      we want: 
-      U'[eT'/x] ->n sU'
-
-
-      we have (subst lemma)
-      U[eT/x] ->* normalized(U'[eT'/x])
-
-      and U[eT/x] ->| sU'
-
-      by triangle lemma
-      U'[eT'/x] ->| sU'
-      but we need that normalization is enough
-
-
-      Steps after sub can be done before
-      and no relevant step contradicted by subst
-      but:
-      argument is a lambda => creates redex after subst
-
-
-
-      by uniqueness of normalization, this is sU'
-
-
-
-
-      idea:
-      sU does all its eval steps in eT' and the one in U
-      TODO: why no overlap => why not sub into b? (e.g. why are U subst sites not destroyed)
-
-      b does not change eT 
-      or it is closed in the env of eT
-
-      x free in b:
-        eT' = eT
-
-      x not free in b:
-        subst x does not interfere with eval points (just might add some)
-        i.e. subst x expr b = b
-        statement holds
-
-      if x free:
-        then unify all free vars => anything that is placed in for x can be unified with x => use it
-    *)
-    admit.
-Qed.
-
-
-(*
-
-does not work => we have b steps but know nothing => same problem
-
-Lemma typed_preservation_eventually
-  Γ e A:
-  TY Γ ⊢ e : A →
-  forall e' A' b,
-  e →[b]ᵦₙ* e' →
-  A →[b]ᵦₙ* A' →
-  exists e'' A'',
-  e' →[b]ᵦₙ* e'' ∧
-  A' →[b]ᵦₙ* A'' ∧
-  TY Γ ⊢ e'' : A''.
-Proof.
-  intros HTy. 
-  induction HTy.
-  (* do not step *)
-  1,2,3,4,5,6,7: admit.
-  (* only Pi, Lam, App left *)
-  all: intros e' A' b Hstepe HstepA.
-  - (* Pi *)
-    admit.
-  - (* Lam *)
-    admit.
-  - (* App *)
-    rename e into eA.
-    idtac.
-    assert  (
-      exists eT',
-      eT →[ b ]ᵦₙ* eT' /\ 
-      e' = eA eT'
-    ) as (eT'&HstepeT&->) by admit.
- *)
-
-
-
-(* Lemma typed_preservation_eventually
-  Γ e A:
-  TY Γ ⊢ e : A →
-  forall e',
-  e →ᵦₙ* e' →
-  exists e'' A' A'',
-  A →ᵦₙ* A' ∧
-  e' →ᵦₙ* e'' ∧
-  A' →ᵦₙ* A'' ∧
-  TY Γ ⊢ e'' : A''.
-Proof.
-  intros HTy e' Hstep.
-  induction Hstep.
-  - do 3 eexists. 
-    split;[|split;[|split]].
-    1-3: constructor.
-    assumption.
-  -   
-    enough (
-      ∃ e'' A' A'' : expr, A →ᵦₙ* A' ∧ y →ᵦₙ* e'' ∧ A' →ᵦₙ* A'' ∧ TY Γ ⊢ e'' : A''
-    ).
-    {
-      destruct H0 as (?&?&?&?&?&?&?).
-      do 3 eexists.
-      split;[|split;[|split]].
-      4: apply H3.
-      1,3:eassumption.
-      admit. (* would need confluence *)
-    } 
-Abort. *)
-
-
-(*
-if typed expression takes one step
-than it can take a few more to reach a typed state.
-
-newest generalization:
-if either expression or type steps both step further to a combined finished state
-*)
-Lemma typed_preservation_eventually
-  Γ e A:
-  TY Γ ⊢ e : A →
-  forall e' A',
-  e →ᵦₙ* e' →
-  A →ᵦₙ* A' →
-  exists e'' A'',
-  e' →ᵦₙ* e'' ∧
-  A' →ᵦₙ* A'' ∧
-  TY Γ ⊢ e'' : A''.
-Proof.
-  intros HTy. 
-  induction HTy.
-  (* do not step *)
-  1,2,3,4,5,6,7: admit.
-  (* only Pi, Lam, App left *)
-  all: intros e' A' Hstepe HstepA.
-  - (* Pi *)
-    (*
-      e' = Pi x T' U'
-      s.t.
-      T →ᵦₙ* T'
-      U →ᵦₙ* U'
-
-      by IH we have 
-      typed 
-      T'' and U''
-
-      need env step as U might depend on T
-    *)
-    admit.
-  - (* Lam *)
-    (*
-      Lambda also has no toplevel step but is has dependencies directly 
-
-      each component steps and then steps to adhere to other
-      => maybe our IH is good enough, TODO: check
-
-    *)
-    admit.
-  - (* App *)
-    (*
-      either subcomponent steps or toplevel
-      (or all in different time steps)
-
-      Idea:
-      first step is toplevel
-      or steps before
-      decompose: 
-        both sides step then maybe toplevel, then maybe more
-
-      eT steps to eT' (and T might step somewhere)
-      by IH we get eT'' and T'' s.t.
-      eT'' : T''
-
-      now we know that T steps to T''
-      e steps to e 
-      and Pi x T U to Pi x T'' U
-      then we get 
-
-
-      mh do we need confluence?
-    *)
-    rename e into eA.
-    idtac.
-
-
-
-  (*
-    destruct on context
-  *)
-  
-Admitted.
-
-
-
-
-
-
-
-
-(* Difference to onestep: we have →ᵦ* instead of just one step *)
-Lemma typed_preservation_eventually_invers:
-  (forall Γ e A (H:TY Γ ⊢ e : A),
-  forall (HTy: TY Γ ⊢ e : A), 
-    forall A', A →ᵦ* A' →
-
-    (* we need the same eventual-stepping as types can be as weird as expressions *)
-    exists e' e'' A'' A''',
-    TY Γ ⊢ e'' : A''' ∧
-    (e →ᵦ* e' ∧ e' →ₙ e'') ∧
-    (A' →ᵦ* A'' ∧ A'' →ₙ A''')
-  ).
-Proof.
-(* maybe we need induction over K? *)
-  (* intros ? ? ? H.
-  induction H.
-  all: intros HTy -> A' Hstep.
-  all: destruct Hstep as [K e1 e2 He1 He2 Hstep];subst.
-  all: destruct K;simpl in *;try congruence.
-  all: subst.
-  all: try now inversion Hstep.
-  all: try inversion He1;subst.
-  - admit.
-  - admit.
-  - admit.
-  - admit. *)
-Admitted.
-
-
- Corollary typed_preservation_eventually_invers_onestep:
-  (forall Γ e A (H:TY Γ ⊢ e : A),
-  forall (HTy: TY Γ ⊢ e : A), 
-    forall A', A →ᵦ A' →
-
-    (* we need the same eventual-stepping as types can be as weird as expressions *)
-    exists e' e'' A'' A''',
-    TY Γ ⊢ e'' : A''' ∧
-    (e →ᵦ* e' ∧ e' →ₙ e'') ∧
-    (A' →ᵦ* A'' ∧ A'' →ₙ A''')
-  ).
-Proof.
-Admitted.
-
-
-
-(*
-If expression steps, it is eventually typed again
-*)
-Lemma typed_preservation_eventually:
-  (forall Γ e A (H:TY Γ ⊢ e : A),
-  forall (HTy: TY Γ ⊢ e : A), 
-    (* Γ = ∅ → *)
-    forall e', e →ᵦ e' →
-    exists e'' e''' A' A'',
-    TY Γ ⊢ e''' : A'' ∧
-    (e' →ᵦ* e'' ∧ e'' →ₙ e''') ∧
-    (A →ᵦ* A' ∧ A' →ₙ A'')
-  ).
-Proof.
-  intros ? ? ? H.
-  induction H.
-  all: intros HTy e' Hstep.
-
-  all: destruct Hstep as [K e1 e2 He1 He2 Hstep];subst.
-  all: destruct K;simpl in *;try congruence.
-  all: subst.
-  all: try now inversion Hstep.
-  all: try inversion He1;subst.
-  (* the type of a lam will also come up *)
-  (* also return type => if we have e_{2+2} in the body, the return type changes from Idx (2+2) to Idx(4) *)
-  - (* Pi domain *)
-
-    (* e1 takes one step to e2
-    by IH 
-    fill K e1 takes a few steps until typed again
-
-    extend those steps to Pi 
-    and but is U still typed under this? (in env x:T)
-
-    if step in context => still typed => see paper again (page 58)
-    *)
-    specialize (IHsyn_typed1 H (fill K e2)).
-    edestruct IHsyn_typed1 as (Ke2'&Ke2''&A'&A''&HTyKe2''&(HBKe2&HNKe2)&(HBA'&HN'A)).
-    1: now apply fill_step.
-    assert (TY (insert_name x0 Ke2'' Γ) ⊢ U0 : Sort sU) by admit. (* Assumption step *)
-    (* TODO: U0 already normalized *)
-    (* assert (Pi'' = Pi x0 Ke2'' U0) as -> by admit.
-    assert (exists Pi'', 
-      normal_eval (Pi x0 Ke2' U0) Pi'') as [Pi'' HPi''] by admit. *)
-    assert (
-      normal_eval (Pi x0 Ke2' U0) (Pi x0 Ke2'' U0)
-    ) by admit.
-    assert (A'' = Sort sT) as -> by admit. (* inversion Sort beta, norm *)
-    exists (Pi x0 Ke2' U0).
-    exists (Pi x0 Ke2'' U0).
-    do 2 eexists.
-    split;[|split;split].
-    2-3: admit. (* easy, Pi congruence beta norm *)
-    1: apply typed_pi;eassumption.
-    1-2: admit. (* easy, LitNat beta norm *)
-
-  - (* Pi codomain *)
-    (* specialize (IHsyn_typed2 H0 eq_refl (fill K e2)). *)
-    edestruct IHsyn_typed2 as (Ke2'&Ke2''&A'&A''&HTyKe2''&(HBKe2&HNKe2)&(HBA'&HN'A)).
-    1: assumption.
-    1: eapply fill_step;eassumption.
-    exists (Pi x0 T0 Ke2').
-    exists (Pi x0 T0 Ke2''). (* T0 already normalized *)
-    do 2 exists (LitNat (sT `max` sU)).
-    split;[|split;split].
-    4-5: admit. (* easy LitNat beta norm *)
-    2-3: admit. (* easy Pi beta norm congruence *)
-    constructor.
-    1: eassumption.
-    assert(A'' = Sort sU) as -> by admit. (* Sort inversion beta norm *)
-    assumption.
-
-  - (* domain Type of lambda *)
-  (*
-    same as above:
-    we follow the beta,
-    everything else is normalized and no top-level normalization
-    => just follow subexpression
-  *)
-  (*
-    special as our type recursion is on Pi not T and U
-    still possible (just do 2 beta step chains) but probably individually easier
-  *)
-    specialize (IHsyn_typed1 H (fill K e2)).
-    edestruct IHsyn_typed1 as (Ke2'&Ke2''&A'&A''&HTyKe2''&(HBKe2&HNKe2)&(HBA'&HN'A)).
-    1: now apply fill_step.
-    assert (A'' = Sort sT) as -> by admit. (* Sort inversion beta norm *)
-    exists (Lam x0 Ke2' f U0 e0).
-    exists (Lam x0 Ke2'' f U0 e0).
-    exists (Pi x0 Ke2' U0).
-    exists (Pi x0 Ke2'' U0).
-    split;[|split;split].
-    1: {
-      eapply typed_lam.
-      1: eassumption.
-      all: admit. (* TODO: step in assumption *)
-    }
-    1-2: admit. (* easy *)
-    1-2: admit. (* easy *)
-
-  - (* codomain of Lambda *)
-
-    (*
-      The codomain changes 
-      => body needs to step the change 
-
-      currently, we have preservation as:
-      if expression steps, there is a stepped type
-
-      here, we need
-      if type steps, expression can step too
-
-
-      confluence/church rosser alone would not be enough
-      The statement would be:
-        e moves not has a type resulting from the old one
-        both meet => 
-          we get a new type of body expression (by IH as body steps)
-          by confluence this stepped from the original codomain
-        (we need that it steps at least one time but we can do this by value distinction and contradiction)
-      however, for this we need that the body steps which we do not have
-    *)
-
-
-    (* edestruct IHsyn_typed2 as (Ke2'&Ke2''&A'&A''&HTyKe2''&(HBKe2&HNKe2)&(HBA'&HN'A)).
-    1: eassumption.
-    1: admit. (* extended context *)
-    1: eapply fill_step;eassumption.
-    assert (A'' = Sort sU) as -> by admit. *)
-
-    specialize (typed_preservation_eventually_invers_onestep 
-      (insert_name x0 T0 ∅)
-      e0 
-      (fill K e1)
-      H2 H2 
-    ) as InvPreserve.
-    edestruct InvPreserve as (e0'&e0''&A'&A''&HTye0''&(Hstepe0&Hnorme0)&(HstepA'&HnormA')).
-    1: eapply fill_step;eassumption.
-
-
-    exists (Lam x0 T0 f A'  e0').
-    exists (Lam x0 T0 f A'' e0'').
-    exists (Pi x0 T0 A').
-    exists (Pi x0 T0 A'').
-    split;[|split;split].
-    1: {
-      eapply typed_lam.
-      1: eassumption. (* T did not change *)
-      all: try eassumption. (* f did not change *)
-      (* TODO: A'' is still typed with sort *)
-      admit.
-    }
-
-    all: admit. (* easy *)
-
-  - (* body of lambda *)
-
-    edestruct (IHsyn_typed4) as (Ke2'&Ke2''&A'&A''&HTyKe2''&(HBKe2&HNKe2)&(HBA&HNA)).
-    2: eapply fill_step;eassumption.
-    1: eassumption.
-
-    exists (Lam x0 T0 f A'  Ke2').
-    exists (Lam x0 T0 f A'' Ke2'').
-    exists (Pi x0 T0 A').
-    exists (Pi x0 T0 A'').
-    split;[|split;split].
-    2-5: admit. (* easy *)
-    econstructor.
-    all: try eassumption.
-    admit. (* TODO: A'' still Sort typed *)
-    
-
-  - (* toplevel app *)
-
-    assert(exists e2', e2 →ₙ e2') as [e2' He2'] by admit.
-    specialize (typed_preservation_base_step _ _ _ _ _ HTy Hstep He2') as HTye2'.
-    do 4 eexists.
-    split. 2: split;split.
-    1: eassumption.
-    2: eassumption.
-    1: constructor.
-    1: constructor.
-    admit. (* type already normalized (it is the result of normal_eval) *)
-
-  - (* step in left app *)
-    edestruct (IHsyn_typed1) as (Ke2'&Ke2''&A'&A''&HTyKe2''&(HBKe2&HNKe2)&(HBA&HNA)). 
-    1: assumption.
-    1: eapply fill_step;eassumption.
-    (* 
-    TODO:
-    the lambda domain type might make a step
-    then the argument has to make steps
-
-    or the body (and codomain) changes changing the complete type
-     *)
-     rename U' into substU.
-     (* inversion on beta and normal *)
-     assert(
-      exists T' T'' U' U'',
-      A' = Pi x T' U' /\ 
-      T →ᵦ* T' /\ U →ᵦ* U' /\
-      A'' = Pi x T'' U'' /\ 
-      T' →ₙ T'' /\ U' →ₙ U''
-     ) as  
-     (
-      T'&T''&U'&U''&
-      HA'&
-      HBT&HBU&
-      HA''&
-      HNT&HNU
-     ) by admit.
-     subst.
-     (* the argument steps into an expression 
-     of the correct type
-
-     TODO: we want →ᵦ* and norm of the type not in exists
-      *)
-    specialize (typed_preservation_eventually_invers
-      Γ
-      v2 
-      T
-      H0 H0 
-    ) as InvPreserve.
-    edestruct InvPreserve as (v2'&v2''&T2'&T2''&HTyv2''&(Hstepv2&Hnormv2)&(HstepT2'&HnormT2')).
-    1: eassumption.
-    replace T2'' with T'' in * by admit. 
-      (* 
-      TODO:
-      needs confluence? 
-      but normalization complicated it
-      => do we need beta norm steps and their confluence?
-      *)
-
-
-
-
-    (* assert (
-      exists v2' v2'',
-      TY ∅ ⊢ v2'' : T'' /\
-      v2 →ᵦ* v2' /\ 
-      v2' →ₙ v2''
-    ) as (v2'&v2''&HTyv2&HBv2&HNv2) by admit. *)
-    assert(
-      exists substU'',
-      subst' x v2'' U'' →ₙ substU''
-    ) as (substU''&HsubstU'') by admit.
-    exists (App Ke2' v2').
-    exists (App Ke2'' v2'').
-    exists (subst' x v2' U'). (* not correct instance *)
-    (* exists (subst' x v2'' U'').  *)
-    exists (substU''). 
-    split;[|split;split].
-    2,3,5: admit. (* easy *)
-    2: admit. (* see comment => we have subst normal and want beta of that *)
-    econstructor.
-    1: eassumption.
-    1: eassumption.
-    1: eassumption.
-
-    (*
-    why does the normalized subst expression steps to something that is normalized into
-    the required type
-    => TODO: do we want to combine beta and normalization
-    *)
-
-    (* specialize (typed_preservation_eventually_invers 
-      ∅
-      v2
-      T
-      H0 H0 
-    ) as InvPreserve.
-    edestruct InvPreserve as (e0'&e0''&A'&A''&HTye0''&(Hstepe0&Hnorme0)&(HstepA'&HnormA')). *)
-
-
-
-  - (* step in right app *)
-
-    (*
-      for e1 being a lambda, it would be easy 
-      but e1 is no value
-      => use if type steps, values steps
-
-      but the type does (possibly) many steps
-
-      ~~Problem: e0 might change its return type
-      now we have the complicated situation with intermediate normalization~~
-
-      e0 does not change its type (as e0 just follows the argument type reduction)
-      The problem is that (see below in UB and UN)
-    *)
-
-
-
-
-    edestruct IHsyn_typed2 as (Ke2'&Ke2''&A'&A''&HTyKe2''&(HBKe2&HNKe2)&(HBA&HNA)). 
-    1: assumption.
-    1: eapply fill_step;eassumption.
-
-    (* arg steps and lambda must reciprocate steps *)
-    assert(Pi x T U →ᵦ* Pi x A' U) by admit. (* easy *)
-    assert(Pi x A' U →ᵦ* Pi x A'' U) by admit. (* easy *)
-    (* TODO: not exactly the type to expression lemma but instead multiple steps *)
-
-
-    specialize (typed_preservation_eventually_invers
-      _
-      _ 
-      _
-      H H
-    ) as InvPreserve.
-    edestruct InvPreserve as (e0'&e0''&T2'&T2''&HTyv2''&(Hstepe0&Hnorme0)&(HstepT2'&HnormT2')).
-    1: eassumption.
-
-    (* TODO: confluence? Why exactly these beta steps *)
-    assert (T2'' = Pi x A'' U) as -> by admit.
-
-    (* assert(
-      exists e0' e0'', 
-      TY ∅ ⊢ e0'' : Pi x A'' U /\
-      e0 →ᵦ* e0' /\ e0' →ₙ e0''
-    ) as (e0'&e0''&HTye0&HBe0&HNe0) by admit. *)
-
-
-    exists (App e0' Ke2').
-    exists (App e0'' Ke2'').
-    (* exists (subst' x (fill K e1) U). *)
-    (* eexists. *)
-
-    assert (exists UB UN,
-      (* subst' x (fill K e1) U →ᵦ* UB /\ *)
-      True /\
-      UB →ₙ UN /\
-
-      subst' x Ke2'' U →ₙ UN /\
-      U' →ᵦ* UB
-    ) as 
-      (UB&UN&HBUB&HNU&HUN&HBU').
-    {
-      do 2 eexists.
-      split;[|split;[|split]].
-      3: admit. (* defining property of UN *)
-      (* 
-        UB can be subst x Ke2'' U with more or less normalization points
-        e.g. subst x Ke2' U would be more points
-        however, the normalized form (U') of subst x (fill K e1) U has to reduce to UB (3)
-       *)
-      3: admit.
-      all: admit.
-    }
-
-    (* 
-      subst' x (fill K e1) U →ᵦ* UB /\
-      UB →ₙ UN
-
-      subst' x Ke2'' U →ₙ UN
-      (from eval typing)
-      (uniquely determines UN)
-
-      U' →ᵦ* UB
-    *)
-
-    (* assert (exists sUKe2,
-      subst' x (Ke2'') U →ₙ sUKe2) as (sUKe2&HNsUKe2) by admit. *)
-    (*
-      we want just the beta steps in the normalized expression
-      => need confluence?
-    *)
-    (*
-    exists (subst' x (Ke2'') U). (* could be wrong instance *) 
-    exists (sUKe2).
-    *)
-    exists UB.
-    exists UN.
-    split;[|split;split].
-    1: {
-      econstructor.
-      all: try eassumption.
-      (* admit.  *)
-      (* subst already normalized (else normalize) *)
-    }
-    all: try eassumption.
-    all: admit. (* easy *)
-Admitted.
-
-
-(*
-typed_progress: typed expressions  are value or reducible
-typed_preservation: typed expressions reduce eventually into a type expression
-
-=> every typed expression eventually reduced into a typed value
-(typed expressions don't get stuck)
-
-or it loop infinitely
-=> formulation if it terminates, it terminates in a well-typed value
-*)
-
-
-
-
-(* Lemma typed_safety e1 e2 A:
-  TY ∅ ⊢ e1 : A →
-  rtc contextual_step e1 e2 →
-  is_val e2 ∨ reducible e2.
-Proof.
-  induction 2; eauto using typed_progress, typed_preservation.
-Qed. *)
